Weidenbach_Book/Watched_Literals/Watched_Literals_Watch_List_Inprocessing.thy
@@ -1,0 +1,193 @@
+theory Watched_Literals_Watch_List_Inprocessing
+  imports Watched_Literals_Watch_List Watched_Literals_List_Inprocessing
+begin
+
+definition simplify_clause_with_unit_st_wl :: \<open>nat \<Rightarrow> 'v twl_st_wl \<Rightarrow> 'v twl_st_wl nres\<close> where
+  \<open>simplify_clause_with_unit_st_wl = (\<lambda>C (M, N, D, NE, UE, NS, US, N0, U0, Q, W). do {
+    ASSERT (C \<in># dom_m N \<and> count_decided M = 0 \<and> D = None );
+    if C \<in> set (get_all_mark_of_propagated M)
+    then RETURN (M, N, D, NE, UE, NS, US, N0, U0, Q, W)
+    else do {
+      let E = mset (N \<propto> C);
+      let irr = irred N C;
+      (b, N) \<leftarrow> simplify_clause_with_unit C M N;
+      if b then
+        RETURN (M, fmdrop C N, D, (if irr then add_mset E else id) NE, (if \<not>irr then add_mset E else id) UE, NS, US, N0, U0, Q, W)
+      else if size (N \<propto> C) = 1
+      then do {
+        let L = ((N \<propto> C) ! 0);
+        RETURN (Propagated L 0 # M, fmdrop C N, D, (if irr then add_mset {#L#} else id) NE, (if \<not>irr then add_mset {#L#} else id)UE, (if irr then add_mset E else id) NS, (if \<not>irr then add_mset E else id)US, N0, U0, add_mset (-L) Q, W)}
+      else if size (N \<propto> C) = 0
+        then RETURN (M, fmdrop C N, Some {#}, NE, UE, (if irr then add_mset E else id) NS, (if \<not>irr then add_mset E else id) US, (if irr then add_mset {#} else id) N0, (if \<not>irr then add_mset {#} else id)U0, {#}, W)
+      else
+          RETURN (M, N, D, NE, UE, (if irr then add_mset E else id) NS, (if \<not>irr then add_mset E else id) US, N0, U0, Q, W)
+    }
+     })\<close>
+
+definition simplify_clauses_with_unit_st_wl_pre where
+  \<open>simplify_clauses_with_unit_st_wl_pre S \<longleftrightarrow> (\<exists>T.
+  (S, T) \<in> state_wl_l None \<and>
+  set_mset (dom_m (get_clauses_wl S)) \<subseteq>
+    clauses_pointed_to (set_mset (all_init_lits_of_wl S))
+    (get_watched_wl S) \<and>
+  simplify_clauses_with_unit_st_pre T)\<close>
+
+definition simplify_clauses_with_unit_st_wl_inv where
+  \<open>simplify_clauses_with_unit_st_wl_inv S\<^sub>0 it S \<longleftrightarrow> (\<exists>T\<^sub>0 T.
+  (S\<^sub>0, T\<^sub>0) \<in> state_wl_l None \<and>
+  (S, T) \<in> state_wl_l None \<and>
+  simplify_clauses_with_unit_st_inv T\<^sub>0 it T \<and>
+  set_mset (dom_m (get_clauses_wl S)) \<subseteq>
+  clauses_pointed_to (set_mset (all_init_lits_of_wl S))
+  (get_watched_wl S))\<close>
+
+definition simplify_clauses_with_unit_st_wl :: \<open>'v twl_st_wl \<Rightarrow> 'v twl_st_wl nres\<close>  where
+  \<open>simplify_clauses_with_unit_st_wl S =
+  do {
+    ASSERT(simplify_clauses_with_unit_st_wl_pre S);
+    xs \<leftarrow> SPEC(\<lambda>xs. xs \<subseteq>set_mset (dom_m (get_clauses_wl S)));
+    FOREACHci(\<lambda>it T. simplify_clauses_with_unit_st_wl_inv S it T)
+    (xs)
+    (\<lambda>S. get_conflict_wl S = None)
+    (\<lambda>i S. simplify_clause_with_unit_st_wl i S)
+    S
+  }\<close>
+lemma clauses_pointed_to_union:
+  \<open>clauses_pointed_to (A \<union> B) W = clauses_pointed_to A W \<union> clauses_pointed_to B W\<close>
+  by (auto simp: clauses_pointed_to_def)
+
+lemma clauses_pointed_to_mono: \<open>A \<subseteq> B \<Longrightarrow> clauses_pointed_to A W \<subseteq> clauses_pointed_to B W\<close>
+  by (auto simp: clauses_pointed_to_def)
+ 
+lemma simplify_clause_with_unit_st_wl_simplify_clause_with_unit_st:
+  assumes ST: \<open>(S, T) \<in> state_wl_l None\<close> and \<open>(i,j) \<in> nat_rel\<close> and
+    point: \<open>set_mset (dom_m (get_clauses_wl S)) \<subseteq>
+      clauses_pointed_to (set_mset (all_init_lits_of_wl S))
+      (get_watched_wl S)\<close>
+  shows
+  \<open>simplify_clause_with_unit_st_wl i S \<le> \<Down> {(S,T). (S,T) \<in> state_wl_l None \<and>
+    set_mset (dom_m (get_clauses_wl S)) \<subseteq>
+    clauses_pointed_to (set_mset (all_init_lits_of_wl S))
+    (get_watched_wl S)}
+  (simplify_clause_with_unit_st j T)\<close>
+proof -
+  have Id: \<open>A = B \<Longrightarrow> A \<le> \<Down>Id B\<close> for A B
+    by auto
+  have ij: \<open>i = j\<close>
+    using assms by auto
+  have [simp]:
+    \<open>irred b j \<Longrightarrow> j \<in># dom_m b \<Longrightarrow> add_mset (mset (b \<propto> j))
+    ({#mset (fst x). x \<in># remove1_mset (the (fmlookup b j)) (init_clss_l b)#} + d + f + h) =
+    ({#mset (fst x). x \<in># (init_clss_l b)#} + d + f + h)\<close> for C D d b f h j
+    by (auto simp: image_mset_remove1_mset_if ran_m_def
+      dest!: multi_member_split)
+  have H: \<open>fmdrop j x2 = fmdrop j b \<Longrightarrow>
+    mset (x2 \<propto> j) \<subseteq># mset (b \<propto> j) \<Longrightarrow>
+    irred x2 j \<Longrightarrow>
+    irred b j \<Longrightarrow>
+    j \<in># dom_m b \<Longrightarrow>
+    j \<in># dom_m x2 \<Longrightarrow>
+    set_mset (all_lits_of_mm (add_mset (mset (b \<propto> j)) ({#mset (fst x). x \<in># init_clss_l x2#} +
+    d + f + h))) =
+    set_mset (all_lits_of_mm ({#mset (fst x). x \<in># init_clss_l b#} + d + f + h))\<close>
+    for j x2 b d f h
+    using distinct_mset_dom[of x2] distinct_mset_dom[of b]
+    apply (subgoal_tac \<open>{#mset (fst x). x \<in># filter_mset snd {#the (fmlookup b x). x \<in># remove1_mset j (dom_m b)#}#} =
+      {#mset (fst x). x \<in># filter_mset snd {#the (fmlookup x2 x). x \<in># remove1_mset j (dom_m x2)#} #}\<close>)
+
+    apply (auto 5 3 simp: ran_m_def all_lits_of_mm_add_mset
+      dest!: multi_member_split[of _ \<open>dom_m _\<close>]
+      dest: all_lits_of_m_mono
+      intro!: image_mset_cong2 filter_mset_cong2)
+    apply (metis fmdrop_eq_update_eq fmupd_lookup union_single_eq_member)
+    by (metis add_mset_remove_trivial dom_m_fmdrop) 
+
+  show ?thesis
+    supply [[goals_limit=1]]
+    using ST point
+    apply (cases S; hypsubst)
+    apply (cases T; hypsubst)
+    unfolding simplify_clause_with_unit_st_wl_def simplify_clause_with_unit_st_def ij
+      state_wl_l_def prod.simps
+    apply refine_rcg
+    subgoal by auto
+    subgoal by auto
+    subgoal by auto
+    subgoal by auto
+    subgoal by auto
+      apply (rule Id)
+      subgoal by auto
+      subgoal by auto
+      subgoal by (auto simp: all_init_lits_of_wl_def init_clss_l_fmdrop
+        init_clss_l_fmdrop_irrelev
+        dest: in_diffD)
+      subgoal by auto
+      subgoal apply (auto simp: all_init_lits_of_wl_def init_clss_l_fmdrop
+        init_clss_l_fmdrop_irrelev add_mset_commute
+        dest: in_diffD)
+        apply (subst add_mset_commute)
+        apply (auto simp: all_lits_of_mm_add_mset clauses_pointed_to_union
+          dest: in_diffD)
+        done
+      subgoal by auto
+      subgoal by (auto simp: all_init_lits_of_wl_def init_clss_l_fmdrop
+        init_clss_l_fmdrop_irrelev all_lits_of_mm_add_mset
+        dest: in_diffD)
+      subgoal for a b c d e f g h i ja k aa ba ca da ea fa ga ha ia jaa ka x x' x1 x2 x1a x2a
+        
+        apply
+        (auto simp: all_init_lits_of_wl_def init_clss_l_fmdrop
+        init_clss_l_fmdrop_irrelev H
+        dest: in_diffD
+          intro: )
+        apply (metis (no_types, lifting) basic_trans_rules(31) dom_m_fmdrop insert_DiffM) 
+        by (metis (no_types, lifting) basic_trans_rules(31) dom_m_fmdrop init_clss_l_fmdrop_irrelev insert_DiffM)
+      done
+qed
+
+
+lemma simplify_clauses_with_unit_st_wl_simplify_clause_with_unit_st:
+  assumes ST: \<open>(S, T) \<in> state_wl_l None\<close> and
+    point: \<open>set_mset (dom_m (get_clauses_wl S)) \<subseteq>
+    clauses_pointed_to (set_mset (all_init_lits_of_wl S))
+    (get_watched_wl S)\<close>
+  shows
+    \<open>simplify_clauses_with_unit_st_wl S \<le> \<Down> {(S,T). (S,T) \<in> state_wl_l None \<and>
+    set_mset (dom_m (get_clauses_wl S)) \<subseteq>
+    clauses_pointed_to (set_mset (all_init_lits_of_wl S))
+    (get_watched_wl S)}
+    (simplify_clauses_with_unit_st T)\<close>
+proof -
+  have [refine0]: \<open>inj_on id xs\<close> for xs
+    by auto
+  show ?thesis
+    unfolding simplify_clauses_with_unit_st_wl_def simplify_clauses_with_unit_st_def
+    apply (refine_vcg simplify_clause_with_unit_st_wl_simplify_clause_with_unit_st)
+    subgoal
+      using assms unfolding simplify_clauses_with_unit_st_wl_pre_def
+      by blast
+    subgoal
+      using ST by auto
+    subgoal
+      by auto
+    subgoal
+      using assms unfolding simplify_clauses_with_unit_st_wl_pre_def by auto
+    subgoal
+      by auto
+    subgoal for xs xsa it \<sigma> it' \<sigma>'
+      using assms apply -
+      unfolding simplify_clauses_with_unit_st_wl_inv_def
+      apply (rule exI[of _ T])
+      apply (rule exI[of _ \<sigma>'])
+      by auto
+    subgoal
+      by auto
+    subgoal
+      by auto
+    subgoal
+      by auto
+    done
+qed
+
+
+end
