Weidenbach_Book/Watched_Literals/Watched_Literals_Watch_List_Reduce.thy
@@ -1,0 +1,1880 @@
+theory Watched_Literals_Watch_List_Reduce
+  imports Watched_Literals_List_Reduce Watched_Literals_Watch_List
+begin
+no_notation funcset (infixr "\<rightarrow>" 60)
+
+lemma cdcl_twl_restart_get_all_init_clss:
+  assumes \<open>cdcl_twl_restart S T\<close>
+  shows \<open>get_all_init_clss T = get_all_init_clss S\<close>
+  using assms by (induction rule: cdcl_twl_restart.induct) auto
+
+lemma rtranclp_cdcl_twl_restart_get_all_init_clss:
+  assumes \<open>cdcl_twl_restart\<^sup>*\<^sup>* S T\<close>
+  shows \<open>get_all_init_clss T = get_all_init_clss S\<close>
+  using assms by (induction rule: rtranclp_induct) (auto simp: cdcl_twl_restart_get_all_init_clss)
+
+
+text \<open>As we have a specialised version of \<^term>\<open>correct_watching\<close>, we defined a special version for
+the inclusion of the domain:\<close>
+
+definition all_init_lits :: \<open>(nat, 'v literal list \<times> bool) fmap \<Rightarrow> 'v literal multiset multiset \<Rightarrow>
+   'v literal multiset\<close> where
+  \<open>all_init_lits S NUE = all_lits_of_mm ((\<lambda>C. mset C) `# init_clss_lf S + NUE)\<close>
+
+lemma all_init_lits_alt_def:
+  \<open>all_init_lits S (NUE + NUS + N0S) = all_lits_of_mm ((\<lambda>C. mset C) `# init_clss_lf S + NUE + NUS + N0S)\<close>
+  \<open>all_init_lits b (d + f + g) = all_lits_of_mm ({#mset (fst x). x \<in># init_clss_l b#} + d + f + g)\<close>
+  by (auto simp: all_init_lits_def ac_simps)
+
+(* abbreviation all_init_lits_of_wl :: \<open>'v twl_st_wl \<Rightarrow> 'v literal multiset\<close> where
+ *   \<open>all_init_lits_of_wl S \<equiv> all_init_lits (get_clauses_wl S)
+ *     (get_unit_init_clss_wl S + get_subsumed_init_clauses_wl S + get_init_clauses0_wl S)\<close> *)
+
+definition all_init_atms :: \<open>_ \<Rightarrow> _ \<Rightarrow> 'v multiset\<close> where
+  \<open>all_init_atms N NUE = atm_of `# all_init_lits N NUE\<close>
+
+declare all_init_atms_def[symmetric, simp]
+
+lemma all_init_atms_alt_def:
+  \<open>set_mset (all_init_atms N NE) = atms_of_mm (mset `# init_clss_lf N) \<union> atms_of_mm NE\<close>
+  unfolding all_init_atms_def all_init_lits_def
+  by (auto simp: in_all_lits_of_mm_ain_atms_of_iff
+      all_lits_of_mm_def atms_of_ms_def image_UN
+      atms_of_def
+    dest!: multi_member_split[of \<open>(_, _)\<close> \<open>ran_m N\<close>]
+    dest: multi_member_split atm_of_lit_in_atms_of
+    simp del: set_image_mset)
+
+lemma in_set_all_init_atms_iff:
+  \<open>y \<in># all_init_atms bu bw \<longleftrightarrow>
+    y \<in> atms_of_mm (mset `# init_clss_lf bu) \<or> y \<in> atms_of_mm bw\<close>
+  by (auto simp: all_lits_def atm_of_all_lits_of_mm all_init_atms_alt_def atms_of_def
+        in_all_lits_of_mm_ain_atms_of_iff all_lits_of_mm_def atms_of_ms_def image_UN
+    dest!: multi_member_split[of \<open>(_, _)\<close> \<open>ran_m N\<close>]
+    dest: multi_member_split atm_of_lit_in_atms_of
+    simp del: set_image_mset)
+
+lemma all_init_atms_fmdrop_add_mset_unit:
+  \<open>C \<in># dom_m baa \<Longrightarrow> irred baa C \<Longrightarrow>
+    all_init_atms (fmdrop C baa) (add_mset (mset (baa \<propto> C)) da) =
+   all_init_atms baa da\<close>
+  \<open>C \<in># dom_m baa \<Longrightarrow> \<not>irred baa C \<Longrightarrow>
+    all_init_atms (fmdrop C baa) da =
+   all_init_atms baa da\<close>
+  by (auto simp del: all_init_atms_def[symmetric]
+    simp: all_init_atms_def all_init_lits_def
+      init_clss_l_fmdrop_irrelev image_mset_remove1_mset_if)
+
+lemma all_init_lits_of_wl_all_lits_st: \<open>set_mset (all_init_lits_of_wl S) \<subseteq> set_mset (all_lits_st S)\<close>
+  unfolding all_lits_st_def all_lits_def all_lits_of_mm_union all_init_lits_of_wl_def
+  apply (subst (2)all_clss_l_ran_m[symmetric])
+  unfolding image_mset_union
+  apply (cases S)
+  apply (auto simp: all_init_lits_def all_lits_def all_lits_of_mm_union)
+  done
+
+text \<open>To ease the proof, we introduce the following ``alternative'' definitions, that only considers
+  variables that are present in the initial clauses (which are never deleted from the set of
+  clauses, but only moved to another component).
+\<close>
+fun correct_watching' :: \<open>'v twl_st_wl \<Rightarrow> bool\<close> where
+  \<open>correct_watching' (M, N, D, NE, UE, NS, US, N0, U0, Q, W) \<longleftrightarrow>
+    (\<forall>L \<in># all_init_lits_of_wl (M, N, D, NE, UE, NS, US, N0, U0, Q, W).
+       distinct_watched (W L) \<and>
+       (\<forall>(i, K, b)\<in>#mset (W L).
+             i \<in># dom_m N \<longrightarrow> K \<in> set (N \<propto> i) \<and> K \<noteq> L \<and> correctly_marked_as_binary N (i, K, b)) \<and>
+       (\<forall>(i, K, b)\<in>#mset (W L).
+             b \<longrightarrow> i \<in># dom_m N) \<and>
+        filter_mset (\<lambda>i. i \<in># dom_m N) (fst `# mset (W L)) =
+          clause_to_update L (M, N, D, NE, UE, NS, US, N0, U0, {#}, {#}))\<close>
+
+fun correct_watching'' :: \<open>'v twl_st_wl \<Rightarrow> bool\<close> where
+  \<open>correct_watching'' (M, N, D, NE, UE, NS, US, N0, U0, Q, W) \<longleftrightarrow>
+    (\<forall>L \<in># all_init_lits_of_wl (M, N, D, NE, UE, NS, US, N0, U0, Q, W).
+       distinct_watched (W L) \<and>
+       (\<forall>(i, K, b)\<in>#mset (W L).
+             i \<in># dom_m N \<longrightarrow> K \<in> set (N \<propto> i) \<and> K \<noteq> L) \<and>
+        filter_mset (\<lambda>i. i \<in># dom_m N) (fst `# mset (W L)) =
+          clause_to_update L (M, N, D, NE, UE, NS, US, N0, U0, {#}, {#}))\<close>
+
+lemma correct_watching'_correct_watching'': \<open>correct_watching' S \<Longrightarrow> correct_watching'' S\<close>
+  by (cases S) auto
+
+declare correct_watching'.simps[simp del] correct_watching''.simps[simp del]
+
+definition blits_in_\<L>\<^sub>i\<^sub>n' :: \<open>'v twl_st_wl \<Rightarrow> bool\<close> where
+  \<open>blits_in_\<L>\<^sub>i\<^sub>n' S \<longleftrightarrow>
+    (\<forall>L \<in># all_init_lits_of_wl S.
+      \<forall>(i, K, b) \<in> set (watched_by S L). K \<in># all_init_lits_of_wl S)\<close>
+
+definition literals_are_\<L>\<^sub>i\<^sub>n' :: \<open>'v twl_st_wl \<Rightarrow> bool\<close> where
+  \<open>literals_are_\<L>\<^sub>i\<^sub>n' S \<equiv>
+    set_mset (all_learned_lits_of_wl S) \<subseteq> set_mset (all_init_lits_of_wl S) \<and>
+     blits_in_\<L>\<^sub>i\<^sub>n' S\<close>
+
+definition all_init_atms_st :: \<open>'v twl_st_wl \<Rightarrow> 'v multiset\<close> where
+  \<open>all_init_atms_st S \<equiv> all_init_atms (get_clauses_wl S)
+    (get_unit_init_clss_wl S + get_subsumed_init_clauses_wl S + get_init_clauses0_wl S)\<close>
+
+lemma all_init_atms_st_alt_def: \<open>all_init_atms_st S = atm_of `# all_init_lits_of_wl S\<close>
+  by (auto simp: all_atms_def all_lits_st_def all_init_atms_st_def all_init_lits_of_wl_def
+    atm_of_all_lits_of_mm all_init_atms_def all_init_lits_def ac_simps
+    simp del: all_init_atms_def[symmetric])
+
+lemma \<L>\<^sub>a\<^sub>l\<^sub>l_all_init_atms:
+  \<open>set_mset (\<L>\<^sub>a\<^sub>l\<^sub>l (all_init_atms N NU)) = set_mset (all_init_lits N NU)\<close>
+  \<open>set_mset (\<L>\<^sub>a\<^sub>l\<^sub>l (all_init_atms_st S)) = set_mset (all_init_lits_of_wl S)\<close>
+  by (simp_all add: \<L>\<^sub>a\<^sub>l\<^sub>l_atm_of_all_lits_of_mm all_init_atms_def all_init_lits_def
+    all_init_lits_of_wl_def ac_simps all_init_atms_st_def)
+
+lemma literals_are_\<L>\<^sub>i\<^sub>n_cong:
+  \<open>set_mset \<A> = set_mset \<B> \<Longrightarrow> literals_are_\<L>\<^sub>i\<^sub>n \<A> S = literals_are_\<L>\<^sub>i\<^sub>n \<B> S\<close>
+  using \<L>\<^sub>a\<^sub>l\<^sub>l_cong[of \<A> \<B>]
+  unfolding literals_are_\<L>\<^sub>i\<^sub>n_def blits_in_\<L>\<^sub>i\<^sub>n_def is_\<L>\<^sub>a\<^sub>l\<^sub>l_def
+  by auto
+
+lemma all_learned_lits_of_wl_all_lits_st:
+  \<open>set_mset (all_learned_lits_of_wl S) \<subseteq> set_mset (all_lits_st S)\<close>
+  unfolding all_learned_lits_of_wl_def all_lits_st_def all_lits_def
+  apply (subst (2) all_clss_l_ran_m[symmetric])
+  unfolding image_mset_union
+  by (cases S) (auto simp: all_lits_of_mm_union)
+
+lemma all_lits_st_init_learned:
+  \<open>set_mset (all_lits_st S) = set_mset (all_init_lits_of_wl S) \<union> set_mset (all_learned_lits_of_wl S)\<close>
+  unfolding all_learned_lits_of_wl_def all_lits_st_def all_lits_def all_init_lits_of_wl_def
+  apply (subst (1) all_clss_l_ran_m[symmetric])
+  unfolding image_mset_union
+  by (cases S) (auto simp: all_lits_of_mm_union)
+
+lemma \<L>\<^sub>a\<^sub>l\<^sub>l_all_atms:
+  \<open>set_mset (\<L>\<^sub>a\<^sub>l\<^sub>l (all_atms_st S)) = set_mset (all_lits_st S)\<close>
+  by (metis \<L>\<^sub>a\<^sub>l\<^sub>l_atm_of_all_lits_of_mm all_atms_st_alt_def_sym all_lits_def all_lits_st_def)
+
+lemma literals_are_\<L>\<^sub>i\<^sub>n'_literals_are_\<L>\<^sub>i\<^sub>n_iff:
+  assumes
+    Sx: \<open>(S, x) \<in> state_wl_l None\<close> and
+    x_xa: \<open>(x, xa) \<in> twl_st_l None\<close> and
+    struct_invs: \<open>twl_struct_invs xa\<close>
+  shows
+    \<open>literals_are_\<L>\<^sub>i\<^sub>n' S \<longleftrightarrow> literals_are_\<L>\<^sub>i\<^sub>n (all_atms_st S) S\<close> (is ?A)
+    \<open>literals_are_\<L>\<^sub>i\<^sub>n' S \<longleftrightarrow> literals_are_\<L>\<^sub>i\<^sub>n (all_atms_st S) S\<close> (is ?B)
+    \<open>set_mset (all_init_atms_st S) = set_mset (all_atms_st S)\<close> (is ?C) and
+    \<open>set_mset (all_init_lits_of_wl S) = set_mset (all_lits_st S)\<close> (is ?D)
+proof -
+  have \<open>cdcl\<^sub>W_restart_mset.no_strange_atm (state\<^sub>W_of xa)\<close>
+    using struct_invs unfolding twl_struct_invs_def cdcl\<^sub>W_restart_mset.cdcl\<^sub>W_all_struct_inv_def
+      pcdcl_all_struct_invs_def state\<^sub>W_of_def
+    by fast+
+  then have \<open>\<And>L. L \<in> atm_of ` lits_of_l (get_trail_wl S) \<Longrightarrow> L \<in> atms_of_ms
+      ((\<lambda>x. mset (fst x)) ` {a. a \<in># ran_m (get_clauses_wl S) \<and> snd a}) \<union>
+      atms_of_mm (get_unit_init_clss_wl S) \<union>
+      atms_of_mm (get_subsumed_init_clauses_wl S) \<union>
+      atms_of_mm (get_init_clauses0_wl S)\<close> and
+    alien_learned: \<open>atms_of_mm (learned_clss (state\<^sub>W_of xa))
+      \<subseteq> atms_of_mm (init_clss (state\<^sub>W_of xa))\<close>
+    using Sx x_xa unfolding cdcl\<^sub>W_restart_mset.no_strange_atm_def
+    by (auto 5 2 simp add: twl_st twl_st_l twl_st_wl)
+
+  show 1: \<open>set_mset (all_init_lits_of_wl S) = set_mset (all_lits_st S)\<close>
+    unfolding all_lits_st_def all_lits_def all_init_lits_of_wl_def
+    apply (subst (2) all_clss_l_ran_m[symmetric])
+    using alien_learned Sx x_xa
+    unfolding image_mset_union all_lits_of_mm_union
+    by (auto simp : in_all_lits_of_mm_ain_atms_of_iff get_unit_clauses_wl_alt_def
+      twl_st twl_st_l twl_st_wl get_learned_clss_wl_def)
+  have \<open>set_mset (all_init_lits_of_wl S) = set_mset (\<L>\<^sub>a\<^sub>l\<^sub>l (all_init_atms_st S))\<close>
+    unfolding \<L>\<^sub>a\<^sub>l\<^sub>l_all_init_atms(2) ..
+ show A: \<open>literals_are_\<L>\<^sub>i\<^sub>n' S \<longleftrightarrow> literals_are_\<L>\<^sub>i\<^sub>n (all_atms_st S) S\<close> for \<A>
+  proof -
+    have sub: \<open>set_mset (all_lits_st S) \<subseteq> set_mset (all_init_lits_of_wl S) \<longleftrightarrow>
+      is_\<L>\<^sub>a\<^sub>l\<^sub>l (all_init_atms_st S) (all_lits_st S)\<close>
+     using all_init_lits_of_wl_all_lits_st[of S]
+     unfolding is_\<L>\<^sub>a\<^sub>l\<^sub>l_def \<L>\<^sub>a\<^sub>l\<^sub>l_all_init_atms(2) by auto
+   have \<open>set_mset (all_learned_lits_of_wl S) \<subseteq> set_mset (all_lits_st S) \<longleftrightarrow>
+     is_\<L>\<^sub>a\<^sub>l\<^sub>l (all_atms_st S) (all_lits_st S)\<close>
+     using all_init_lits_of_wl_all_lits_st[of S]
+     unfolding all_lits_st_init_learned is_\<L>\<^sub>a\<^sub>l\<^sub>l_def \<L>\<^sub>a\<^sub>l\<^sub>l_all_atms
+     by auto
+   then show ?thesis
+      unfolding literals_are_\<L>\<^sub>i\<^sub>n'_def
+	literals_are_\<L>\<^sub>i\<^sub>n_def blits_in_\<L>\<^sub>i\<^sub>n_def blits_in_\<L>\<^sub>i\<^sub>n'_def sub
+	all_init_lits_def[symmetric] all_lits_alt_def2[symmetric]
+        all_lits_alt_def[symmetric] all_init_lits_alt_def[symmetric]
+        is_\<L>\<^sub>a\<^sub>l\<^sub>l_def[symmetric] all_init_atms_def[symmetric] 1
+      by simp
+   qed
+
+   show C: ?C
+     using 1 unfolding all_atms_st_alt_def all_init_atms_st_alt_def
+     apply (simp add: 1 del: all_init_atms_def[symmetric])
+     by (metis all_atms_st_alt_def set_image_mset)
+
+  show ?B
+    apply (subst A)
+    ..
+qed
+
+
+lemma GC_remap_all_init_atmsD:
+  \<open>GC_remap (N, x, m) (N', x', m') \<Longrightarrow>
+    all_init_atms N NE + all_init_atms m NE  = all_init_atms N' NE  + all_init_atms m' NE\<close>
+  by (induction rule: GC_remap.induct[split_format(complete)])
+    (auto simp: all_init_atms_def all_init_lits_def init_clss_l_fmdrop_if
+       init_clss_l_fmupd_if image_mset_remove1_mset_if
+    simp del: all_init_atms_def[symmetric]
+    simp flip: image_mset_union all_lits_of_mm_add_mset all_lits_of_mm_union)
+
+lemma rtranclp_GC_remap_all_init_atmsD:
+  \<open>GC_remap\<^sup>*\<^sup>* (N, x, m) (N', x', m') \<Longrightarrow>
+    all_init_atms N NE + all_init_atms m NE  = all_init_atms N' NE  + all_init_atms m' NE\<close>
+  by (induction rule: rtranclp_induct[of r \<open>(_, _, _)\<close> \<open>(_, _, _)\<close>, split_format(complete), of for r])
+    (auto dest: GC_remap_all_init_atmsD)
+
+lemma rtranclp_GC_remap_all_init_atms:
+  \<open>GC_remap\<^sup>*\<^sup>* (x1a, Map.empty, fmempty) (fmempty, m, x1ad) \<Longrightarrow>
+    all_init_atms x1ad NE = all_init_atms x1a NE\<close>
+  by (auto dest!: rtranclp_GC_remap_all_init_atmsD[of _ _ _ _ _ _ NE])
+
+lemma GC_remap_all_init_lits:
+  \<open>GC_remap (N, m, new) (N', m', new') \<Longrightarrow>
+    all_init_lits N NE + all_init_lits new NE = all_init_lits N' NE + all_init_lits new' NE\<close>
+  by (induction rule: GC_remap.induct[split_format(complete)])
+    (case_tac \<open>irred N C\<close> ; auto simp: all_init_lits_def init_clss_l_fmupd_if image_mset_remove1_mset_if
+    simp flip: all_lits_of_mm_union)
+
+lemma rtranclp_GC_remap_all_init_lits:
+  \<open>GC_remap\<^sup>*\<^sup>* (N, m, new) (N', m', new') \<Longrightarrow>
+  all_init_lits N NE + all_init_lits new NE = all_init_lits N' NE + all_init_lits new' NE\<close>
+  by (induction rule: rtranclp_induct[of r \<open>(_, _, _)\<close> \<open>(_, _, _)\<close>, split_format(complete), of for r])
+    (auto dest: GC_remap_all_init_lits)
+
+lemma subsumed_clauses_alt_def:
+  \<open>subsumed_clauses S = subsumed_init_clauses S + subsumed_learned_clauses S\<close>
+  by (cases S) auto
+(*
+lemma cdcl_twl_restart_is_\<L>\<^sub>a\<^sub>l\<^sub>l:
+  assumes
+    ST: \<open>cdcl_twl_restart\<^sup>*\<^sup>* S T\<close> and
+    struct_invs_S: \<open>twl_struct_invs S\<close> and
+    L: \<open>is_\<L>\<^sub>a\<^sub>l\<^sub>l \<A> (all_lits_of_st S)\<close>
+  shows  \<open>is_\<L>\<^sub>a\<^sub>l\<^sub>l \<A> (all_lits_of_st T)\<close>
+proof -
+  have \<open>twl_struct_invs T\<close>
+    using rtranclp_cdcl_twl_restart_twl_struct_invs[OF ST struct_invs_S] .
+  then have \<open>cdcl\<^sub>W_restart_mset.no_strange_atm (state\<^sub>W_of T)\<close>
+    unfolding twl_struct_invs_def cdcl\<^sub>W_restart_mset.cdcl\<^sub>W_all_struct_inv_def
+      pcdcl_all_struct_invs_def state\<^sub>W_of_def
+    by fast+
+
+  then have \<open>?thesis \<longleftrightarrow> is_\<L>\<^sub>a\<^sub>l\<^sub>l \<A> (all_lits_of_st T)\<close>
+    unfolding cdcl\<^sub>W_restart_mset.no_strange_atm_def is_\<L>\<^sub>a\<^sub>l\<^sub>l_alt_def
+      subsumed_clauses_alt_def
+    by (cases T)
+      (auto simp: cdcl\<^sub>W_restart_mset_state Un_assoc all_lits_of_st_def all_lits_def)
+  moreover have \<open>get_all_init_clss T = get_all_init_clss S\<close>
+    using rtranclp_cdcl_twl_restart_get_all_init_clss[OF ST] .
+  moreover {
+    have \<open>cdcl\<^sub>W_restart_mset.no_strange_atm (state\<^sub>W_of S)\<close>
+      using struct_invs_S
+      unfolding twl_struct_invs_def cdcl\<^sub>W_restart_mset.cdcl\<^sub>W_all_struct_inv_def
+        pcdcl_all_struct_invs_def state\<^sub>W_of_def
+      by fast+
+    then have \<open>is_\<L>\<^sub>a\<^sub>l\<^sub>l \<A> (all_lits_of_st S)\<close>
+      using L
+      unfolding cdcl\<^sub>W_restart_mset.no_strange_atm_def is_\<L>\<^sub>a\<^sub>l\<^sub>l_alt_def
+      by (cases S)
+        (auto simp: cdcl\<^sub>W_restart_mset_state)
+  }
+  ultimately show ?thesis
+sledgehammer
+    by argo
+qed
+
+
+lemma cdcl_twl_restart_is_\<L>\<^sub>a\<^sub>l\<^sub>l':
+  assumes
+    ST: \<open>cdcl_twl_restart\<^sup>*\<^sup>* S T\<close> and
+    struct_invs_S: \<open>twl_struct_invs S\<close> and
+    L: \<open>is_\<L>\<^sub>a\<^sub>l\<^sub>l \<A> (all_lits_of_mm (get_all_init_clss S))\<close>
+  shows  \<open>is_\<L>\<^sub>a\<^sub>l\<^sub>l \<A> (all_lits_of_mm (get_all_init_clss T))\<close>
+proof -
+  have \<open>twl_struct_invs T\<close>
+    using rtranclp_cdcl_twl_restart_twl_struct_invs[OF ST struct_invs_S] .
+  then have \<open>cdcl\<^sub>W_restart_mset.no_strange_atm (state\<^sub>W_of T)\<close>
+    unfolding twl_struct_invs_def cdcl\<^sub>W_restart_mset.cdcl\<^sub>W_all_struct_inv_def
+        pcdcl_all_struct_invs_def state\<^sub>W_of_def
+    by fast+
+  then have \<open>?thesis \<longleftrightarrow> is_\<L>\<^sub>a\<^sub>l\<^sub>l \<A> (all_lits_of_mm (get_all_init_clss T))\<close>
+    unfolding cdcl\<^sub>W_restart_mset.no_strange_atm_def is_\<L>\<^sub>a\<^sub>l\<^sub>l_alt_def
+    by (cases T)
+      (auto simp: cdcl\<^sub>W_restart_mset_state)
+  moreover have \<open>get_all_init_clss T = get_all_init_clss S\<close>
+    using rtranclp_cdcl_twl_restart_get_all_init_clss[OF ST] .
+  then show ?thesis
+    using L
+    by argo
+qed
+*)
+
+definition remove_all_annot_true_clause_imp_wl_inv
+  :: \<open>'v twl_st_wl \<Rightarrow> _ \<Rightarrow> nat \<times> 'v twl_st_wl \<Rightarrow> bool\<close>
+where
+  \<open>remove_all_annot_true_clause_imp_wl_inv S xs = (\<lambda>(i, T).
+     correct_watching'' S \<and> correct_watching'' T \<and> literals_are_\<L>\<^sub>i\<^sub>n' S \<and> literals_are_\<L>\<^sub>i\<^sub>n' T \<and>
+     (\<exists>S' T'. (S, S') \<in> state_wl_l None \<and> (T, T') \<in> state_wl_l None \<and>
+        remove_all_annot_true_clause_imp_inv S' xs (i, T')))\<close>
+
+definition drop_clause_add_move_init_wl :: \<open>'v twl_st_wl \<Rightarrow> nat \<Rightarrow> 'v twl_st_wl\<close> where
+  \<open>drop_clause_add_move_init_wl = (\<lambda>(M, N, D, NE0, UE, NS, US, N0, U0, Q, W) C.
+     (M, fmdrop C N, D, add_mset (mset (N \<propto> C)) NE0, UE, NS, {#}, N0, U0, Q, W))\<close>
+
+definition drop_clause_wl :: \<open>'v twl_st_wl \<Rightarrow> nat \<Rightarrow> 'v twl_st_wl\<close> where
+  \<open>drop_clause_wl = (\<lambda>(M, N, D, NE0, UE, NS, US, N0, U0, Q, W) C.
+     (M, fmdrop C N, D, NE0, UE, NS, {#}, N0, U0, Q, W))\<close>
+
+definition remove_all_annot_true_clause_one_imp_wl
+  :: \<open>nat \<times> 'v twl_st_wl \<Rightarrow> 'v twl_st_wl nres\<close>
+where
+\<open>remove_all_annot_true_clause_one_imp_wl = (\<lambda>(C, S). do {
+      if C \<in># dom_m (get_clauses_wl S) then
+        if irred (get_clauses_wl S) C
+        then RETURN (drop_clause_add_move_init_wl S C)
+        else RETURN (drop_clause_wl S C)
+      else do {
+        RETURN S
+      }
+  })\<close>
+
+definition remove_all_annot_true_clause_imp_wl
+  :: \<open>'v literal \<Rightarrow> 'v twl_st_wl \<Rightarrow> ('v twl_st_wl) nres\<close>
+where
+\<open>remove_all_annot_true_clause_imp_wl = (\<lambda>L S. do {
+    let xs = get_watched_wl S L;
+    (_, T) \<leftarrow> WHILE\<^sub>T\<^bsup>\<lambda>(i, T). remove_all_annot_true_clause_imp_wl_inv S xs (i, T)\<^esup>
+      (\<lambda>(i, T). i < length xs)
+      (\<lambda>(i, T). do {
+        ASSERT(i < length xs);
+        let (C, _, _) = xs!i;
+        if C \<in># dom_m (get_clauses_wl T) \<and> length ((get_clauses_wl T) \<propto> C) \<noteq> 2
+        then do {
+          T \<leftarrow> remove_all_annot_true_clause_one_imp_wl (C, T);
+          RETURN (i+1, T)
+        }
+        else
+          RETURN (i+1, T)
+      })
+      (0, S);
+    RETURN T
+  })\<close>
+
+
+
+lemma reduce_dom_clauses_fmdrop:
+  \<open>reduce_dom_clauses N0 N \<Longrightarrow> reduce_dom_clauses N0 (fmdrop C N)\<close>
+  using distinct_mset_dom[of N]
+  by (auto simp: reduce_dom_clauses_def distinct_mset_remove1_All)
+
+lemma all_init_lits_of_wl_simps[simp]:
+  \<open>C \<in># dom_m N \<Longrightarrow> \<not>irred N C \<Longrightarrow>
+  all_init_lits_of_wl (M, fmdrop C N, D, NE, UE, NS, US, N0, U0, Q, W) =
+    all_init_lits_of_wl (M, N, D, NE, UE, NS, US, N0, U0, Q, W)\<close>
+  \<open>NO_MATCH {#} US \<Longrightarrow>
+  all_init_lits_of_wl (M, N, D, NE, UE, NS, US, N0, U0, Q, W) =
+    all_init_lits_of_wl (M, N, D, NE, UE, NS, {#}, N0, U0, Q, W)\<close>
+  \<open>NO_MATCH [] M \<Longrightarrow>
+  all_init_lits_of_wl (M, N, D, NE, UE, NS, US, N0, U0, Q, W) =
+    all_init_lits_of_wl ([], N, D, NE, UE, NS, US, N0, U0, Q, W)\<close>
+  \<open>C \<in># dom_m N \<Longrightarrow> irred N C \<Longrightarrow>
+   all_init_lits_of_wl (M, fmdrop C N, D, add_mset (mset (N \<propto> C)) NE, UE, NS, US, N0, U0, Q, W) =
+  all_init_lits_of_wl (M, N, D, NE, UE, NS, US, N0, U0, Q, W)\<close>
+  \<open>all_init_lits_of_wl (M, N, D, NE, add_mset E UE, NS, US, N0, U0, Q, W) =
+    all_init_lits_of_wl (M, N, D, NE, UE, NS, US, N0, U0, Q, W)\<close>
+  by (auto simp: all_init_lits_of_wl_def all_lits_of_mm_add_mset
+    image_mset_remove1_mset_if)
+
+lemma all_learned_lits_of_wl_simps[simp]:
+  \<open>C \<in># dom_m N \<Longrightarrow> irred N C \<Longrightarrow>
+  all_learned_lits_of_wl (M, fmdrop C N, D, NE, UE, NS, US, N0, U0, Q, W) =
+    all_learned_lits_of_wl (M, N, D, NE, UE, NS, US, N0, U0, Q, W)\<close>
+  (* \<open>NO_MATCH {#} NS \<Longrightarrow>
+   * all_learned_lits_of_wl (M, N, D, NE, UE, NS, US, N0, U0, Q, W) =
+   *   all_learned_lits_of_wl (M, N, D, NE, UE, {#}, US, N0, U0, Q, W)\<close> *)
+  \<open>NO_MATCH [] M \<Longrightarrow>
+  all_learned_lits_of_wl (M, N, D, NE, UE, NS, US, N0, U0, Q, W) =
+    all_learned_lits_of_wl ([], N, D, NE, UE, NS, US, N0, U0, Q, W)\<close>
+  \<open>all_learned_lits_of_wl (M, N, D, add_mset E NE, UE, NS, US, N0, U0, Q, W) =
+    all_learned_lits_of_wl (M, N, D, NE, UE, NS, US, N0, U0, Q, W)\<close>
+  \<open>all_learned_lits_of_wl (M, N, D, NE, UE, add_mset E NS, US, N0, U0, Q, W) =
+    all_learned_lits_of_wl (M, N, D, NE, UE, NS, US, N0, U0, Q, W)\<close>
+  \<open>C \<in># dom_m N \<Longrightarrow> \<not>irred N C \<Longrightarrow>
+  all_learned_lits_of_wl (M, fmdrop C N, D, NE, add_mset (mset (N \<propto> C)) UE, NS, US, N0, U0, Q, W) =
+  all_learned_lits_of_wl (M, N, D, NE, UE, NS, US, N0, U0, Q, W)\<close>
+  by (auto simp: all_learned_lits_of_wl_def all_lits_of_mm_add_mset
+    image_mset_remove1_mset_if)
+
+lemma correct_watching_fmdrop:
+  assumes
+    irred: \<open>\<not> irred N C\<close> and
+    C: \<open>C \<in># dom_m N\<close> and
+    \<open>correct_watching' (M', N, D, NE, UE, NS, US, N0, U0, Q, W)\<close> and
+    C2: \<open>length (N \<propto> C) \<noteq> 2\<close> and
+    blit: \<open>literals_are_\<L>\<^sub>i\<^sub>n' (M', N, D, NE, UE, NS, US, N0, U0, Q, W)\<close>
+  shows \<open>correct_watching' (M, fmdrop C N, D, NE, UE, NS, {#}, N0, U0, Q, W)\<close> and
+     \<open>literals_are_\<L>\<^sub>i\<^sub>n'  (M, fmdrop C N, D, NE, UE, NS, {#}, N0, U0, Q, W)\<close>
+proof -
+  let ?S = \<open>(M', N, D, NE, UE, NS, US, N0, U0, Q, W)\<close>
+  have
+    Hdist: \<open>\<And>L i K b. L\<in>#all_init_lits_of_wl ?S \<Longrightarrow>
+       distinct_watched (W L)\<close> and
+    H1: \<open>\<And>L i K b. L\<in>#all_init_lits_of_wl ?S \<Longrightarrow>
+       (i, K, b)\<in>#mset (W L) \<Longrightarrow> i \<in># dom_m N \<Longrightarrow> K \<in> set (N \<propto> i) \<and> K \<noteq> L \<and>
+         correctly_marked_as_binary N (i, K, b)\<close> and
+    H1': \<open>\<And>L i K b. L\<in>#all_init_lits_of_wl ?S \<Longrightarrow>
+       (i, K, b)\<in>#mset (W L) \<Longrightarrow> b \<Longrightarrow>  i \<in># dom_m N\<close> and
+    H2: \<open>\<And>L. L\<in># all_init_lits_of_wl ?S \<Longrightarrow>
+       {#i \<in># fst `# mset (W L). i \<in># dom_m N#} =
+       {#C \<in># dom_m (get_clauses_l (M', N, D, NE, UE, NS, US, N0, U0, {#}, {#})).
+        L \<in> set (watched_l (get_clauses_l (M', N, D, NE, UE, NS, US, N0, U0, {#}, {#}) \<propto> C))#}\<close>
+    using assms
+    unfolding correct_watching'.simps clause_to_update_def
+    by fast+
+  have 1: \<open>{#Ca \<in># dom_m (fmdrop C N). L \<in> set (watched_l (fmdrop C N \<propto> Ca))#} =
+    {#Ca \<in># dom_m (fmdrop C N). L \<in> set (watched_l (N \<propto> Ca))#}\<close> for L
+    apply (rule filter_mset_cong2)
+      using distinct_mset_dom[of N] C irred
+    by (auto simp: image_mset_remove1_mset_if clause_to_update_def image_filter_replicate_mset
+      distinct_mset_remove1_All filter_mset_neq_cond dest: all_lits_of_mm_diffD
+        dest: multi_member_split)
+  have 2: \<open>remove1_mset C {#Ca \<in># dom_m N. L \<in> set (watched_l (N \<propto> Ca))#} =
+     removeAll_mset C {#Ca \<in># dom_m N. L \<in> set (watched_l (N \<propto> Ca))#}\<close> for L
+    apply (rule distinct_mset_remove1_All)
+    using distinct_mset_dom[of N]
+    by (auto intro: distinct_mset_filter)
+  have [simp]: \<open>filter_mset (\<lambda>i. i \<in># remove1_mset C (dom_m N)) A  =
+    removeAll_mset C (filter_mset (\<lambda>i. i \<in># dom_m N) A)\<close> for A
+    by (induction A)
+      (auto simp: distinct_mset_remove1_All distinct_mset_dom)
+  show  \<open>correct_watching' (M, fmdrop C N, D, NE, UE, NS, {#}, N0, U0, Q, W)\<close>
+    unfolding correct_watching'.simps clause_to_update_def
+    apply (intro conjI impI ballI)
+    subgoal for L using Hdist[of L] distinct_mset_dom[of N]
+        H1[of L \<open>fst iK\<close> \<open>fst (snd iK)\<close> \<open>snd (snd iK)\<close>] C irred
+	H1'[of L \<open>fst iK\<close> \<open>fst (snd iK)\<close> \<open>snd (snd iK)\<close>]
+      apply (auto simp: image_mset_remove1_mset_if clause_to_update_def image_filter_replicate_mset
+      distinct_mset_remove1_All filter_mset_neq_cond correctly_marked_as_binary.simps dest: all_lits_of_mm_diffD
+        dest: multi_member_split)
+      done
+    subgoal for L iK
+      using distinct_mset_dom[of N] H1[of L \<open>fst iK\<close> \<open>fst (snd iK)\<close> \<open>snd (snd iK)\<close>] C irred
+        H1'[of L \<open>fst iK\<close> \<open>fst (snd iK)\<close> \<open>snd (snd iK)\<close>]
+      apply (auto simp: image_mset_remove1_mset_if clause_to_update_def image_filter_replicate_mset
+      distinct_mset_remove1_All filter_mset_neq_cond correctly_marked_as_binary.simps dest: all_lits_of_mm_diffD
+        dest: multi_member_split)
+      done
+    subgoal for L iK
+       using distinct_mset_dom[of N] H1[of L \<open>fst iK\<close> \<open>fst (snd iK)\<close> \<open>snd (snd iK)\<close>] C irred
+        H1'[of L \<open>fst iK\<close> \<open>fst (snd iK)\<close> \<open>snd (snd iK)\<close>] C2
+      apply (auto simp: image_mset_remove1_mset_if clause_to_update_def image_filter_replicate_mset
+      distinct_mset_remove1_All filter_mset_neq_cond correctly_marked_as_binary.simps dest: all_lits_of_mm_diffD
+        dest: multi_member_split)
+      done
+    subgoal for L
+      using C irred apply -
+      unfolding get_clauses_l.simps
+      apply (subst 1)
+      by (auto 5 1  simp: image_mset_remove1_mset_if clause_to_update_def image_filter_replicate_mset
+        distinct_mset_remove1_All filter_mset_neq_cond 2 H2 dest: all_lits_of_mm_diffD
+        dest: multi_member_split)
+    done
+  have [dest!]: \<open>x \<in># all_learned_lits_of_wl ([], fmdrop C N, D, NE, UE, NS, {#}, N0, U0, Q, W) \<Longrightarrow>
+    x \<in># all_learned_lits_of_wl ([], N, D, NE, UE, NS, US, N0, U0, Q, W)\<close> for x
+    using assms(1,2)
+    by (auto dest: all_lits_of_mm_diffD simp: all_learned_lits_of_wl_def all_lits_of_mm_union
+      image_mset_remove1_mset_if)
+
+  show \<open>literals_are_\<L>\<^sub>i\<^sub>n'  (M, fmdrop C N, D, NE, UE, NS, {#}, N0, U0, Q, W)\<close>
+     using assms by (auto simp: blits_in_\<L>\<^sub>i\<^sub>n'_def image_mset_remove1_mset_if literals_are_\<L>\<^sub>i\<^sub>n'_def
+         all_init_lits_def all_lits_of_mm_union
+       dest: multi_member_split all_lits_of_mm_diffD)
+qed
+
+lemma correct_watching''_fmdrop:
+  assumes
+    irred: \<open>\<not> irred N C\<close> and
+    C: \<open>C \<in># dom_m N\<close> and
+    \<open>correct_watching'' (M', N, D, NE, UE, NS, US, N0, U0, Q, W)\<close> and
+    \<open>literals_are_\<L>\<^sub>i\<^sub>n'  (M', N, D, NE, UE, NS, US, N0, U0, Q, W)\<close>
+  shows \<open>correct_watching'' (M, fmdrop C N, D, NE, UE, NS, {#}, N0, U0, Q, W)\<close>and
+    \<open>literals_are_\<L>\<^sub>i\<^sub>n'  (M, fmdrop C N, D, NE, UE, NS, {#}, N0, U0, Q, W)\<close>
+proof -
+  let ?S = \<open>(M', N, D, NE, UE, NS, US, N0, U0, Q, W)\<close>
+  let ?\<L> = \<open>all_init_lits_of_wl ?S\<close>
+  have
+    Hdist: \<open>\<And>L i K b. L\<in>#?\<L> \<Longrightarrow>
+       distinct_watched (W L)\<close> and
+    H1: \<open>\<And>L i K b. L\<in>#?\<L> \<Longrightarrow>
+       (i, K, b)\<in>#mset (W L) \<Longrightarrow> i \<in># dom_m N \<Longrightarrow> K \<in> set (N \<propto> i) \<and> K \<noteq> L\<close> and
+    H2: \<open>\<And>L. L\<in>#?\<L> \<Longrightarrow>
+       {#i \<in># fst `# mset (W L). i \<in># dom_m N#} =
+       {#C \<in># dom_m (get_clauses_l (M', N, D, NE, UE, NS, US,N0, U0,  {#}, {#})).
+        L \<in> set (watched_l (get_clauses_l (M', N, D, NE, UE, NS, US, N0, U0, {#}, {#}) \<propto> C))#}\<close>
+    using assms
+    unfolding correct_watching''.simps clause_to_update_def
+    by fast+
+  have 1: \<open>{#Ca \<in># dom_m (fmdrop C N). L \<in> set (watched_l (fmdrop C N \<propto> Ca))#} =
+    {#Ca \<in># dom_m (fmdrop C N). L \<in> set (watched_l (N \<propto> Ca))#}\<close> for L
+    apply (rule filter_mset_cong2)
+      using distinct_mset_dom[of N] C irred
+    by (auto simp: image_mset_remove1_mset_if clause_to_update_def image_filter_replicate_mset
+      distinct_mset_remove1_All filter_mset_neq_cond dest: all_lits_of_mm_diffD
+        dest: multi_member_split)
+  have 2: \<open>remove1_mset C {#Ca \<in># dom_m N. L \<in> set (watched_l (N \<propto> Ca))#} =
+     removeAll_mset C {#Ca \<in># dom_m N. L \<in> set (watched_l (N \<propto> Ca))#}\<close> for L
+    apply (rule distinct_mset_remove1_All)
+    using distinct_mset_dom[of N]
+    by (auto intro: distinct_mset_filter)
+  have [simp]: \<open>filter_mset (\<lambda>i. i \<in># remove1_mset C (dom_m N)) A  =
+    removeAll_mset C (filter_mset (\<lambda>i. i \<in># dom_m N) A)\<close> for A
+    by (induction A)
+      (auto simp: distinct_mset_remove1_All distinct_mset_dom)
+  show  \<open>correct_watching'' (M, fmdrop C N, D, NE, UE, NS, {#}, N0, U0, Q, W)\<close>
+    unfolding correct_watching''.simps clause_to_update_def
+    apply (intro conjI impI ballI)
+    subgoal for L using Hdist[of L] distinct_mset_dom[of N]
+        H1[of L \<open>fst iK\<close> \<open>fst (snd iK)\<close> \<open>snd (snd iK)\<close>] C irred
+      apply (auto simp: image_mset_remove1_mset_if clause_to_update_def image_filter_replicate_mset
+      distinct_mset_remove1_All filter_mset_neq_cond correctly_marked_as_binary.simps dest: all_lits_of_mm_diffD
+        dest: multi_member_split)
+      done
+    subgoal for L iK
+      using distinct_mset_dom[of N] H1[of L \<open>fst iK\<close> \<open>fst (snd iK)\<close> \<open>snd (snd iK)\<close>] C irred
+      apply (auto simp: image_mset_remove1_mset_if clause_to_update_def image_filter_replicate_mset
+      distinct_mset_remove1_All filter_mset_neq_cond correctly_marked_as_binary.simps dest: all_lits_of_mm_diffD
+        dest: multi_member_split)
+      done
+    subgoal for L
+      using C irred apply -
+      unfolding get_clauses_l.simps
+      apply (subst 1)
+      by (auto 5 1  simp: image_mset_remove1_mset_if clause_to_update_def image_filter_replicate_mset
+        distinct_mset_remove1_All filter_mset_neq_cond 2 H2 dest: all_lits_of_mm_diffD
+        dest: multi_member_split)
+    done
+  have [dest!]: \<open>x \<in># all_learned_lits_of_wl ([], fmdrop C N, D, NE, UE, NS, {#}, N0, U0, Q, W) \<Longrightarrow>
+           x \<in># all_learned_lits_of_wl ([], N, D, NE, UE, NS, US, N0, U0, Q, W)\<close> for x
+    using assms
+    by (auto dest: all_lits_of_mm_diffD simp: all_learned_lits_of_wl_def
+      all_lits_of_mm_union image_mset_remove1_mset_if)
+  show \<open>literals_are_\<L>\<^sub>i\<^sub>n'  (M, fmdrop C N, D, NE, UE, NS, {#}, N0, U0, Q, W)\<close>
+    using assms by (auto simp: blits_in_\<L>\<^sub>i\<^sub>n'_def image_mset_remove1_mset_if literals_are_\<L>\<^sub>i\<^sub>n'_def
+         all_init_lits_def all_lits_of_mm_union
+       dest: multi_member_split all_lits_of_mm_diffD)
+qed
+
+lemma correct_watching''_fmdrop':
+  assumes
+    irred: \<open>irred N C\<close> and
+    C: \<open>C \<in># dom_m N\<close> and
+    \<open>correct_watching'' (M', N, D, NE, UE, NS, US, N0, U0, Q, W)\<close>and
+    \<open>literals_are_\<L>\<^sub>i\<^sub>n' (M', N, D, NE, UE, NS, US, N0, U0, Q, W)\<close>
+  shows \<open>correct_watching'' (M, fmdrop C N, D, add_mset (mset (N \<propto> C)) NE, UE, NS, {#}, N0, U0, Q, W)\<close> and
+    \<open>literals_are_\<L>\<^sub>i\<^sub>n' (M, fmdrop C N, D, add_mset (mset (N \<propto> C)) NE, UE, NS, {#}, N0, U0, Q, W)\<close>
+proof -
+  let ?S = \<open>(M', N, D, NE, UE, NS, US, N0, U0, Q, W)\<close>
+  let ?\<L> = \<open>all_init_lits_of_wl ?S\<close>
+  have
+    Hdist: \<open>\<And>L. L\<in>#?\<L> \<Longrightarrow>
+       distinct_watched (W L)\<close> and
+    H1: \<open>\<And>L i K b. L\<in>#?\<L> \<Longrightarrow>
+       (i, K, b)\<in>#mset (W L) \<Longrightarrow> i \<in># dom_m N \<Longrightarrow>
+          K \<in> set (N \<propto> i) \<and> K \<noteq> L\<close> and
+    H2: \<open>\<And>L. L\<in>#?\<L> \<Longrightarrow>
+       {#i \<in># fst `# mset (W L). i \<in># dom_m N#} =
+       {#C \<in># dom_m (get_clauses_l (M', N, D, NE, UE, NS, US, N0, U0, {#}, {#})).
+        L \<in> set (watched_l (get_clauses_l (M', N, D, NE, UE, NS, US, N0, U0, {#}, {#}) \<propto> C))#}\<close>
+    using assms
+    unfolding correct_watching''.simps clause_to_update_def
+    by blast+
+  have 1: \<open>{#Ca \<in># dom_m (fmdrop C N). L \<in> set (watched_l (fmdrop C N \<propto> Ca))#} =
+    {#Ca \<in># dom_m (fmdrop C N). L \<in> set (watched_l (N \<propto> Ca))#}\<close> for L
+    apply (rule filter_mset_cong2)
+      using distinct_mset_dom[of N] H1[of L \<open>fst iK\<close> \<open>snd iK\<close>] C irred
+    by (auto simp: image_mset_remove1_mset_if clause_to_update_def image_filter_replicate_mset
+      distinct_mset_remove1_All filter_mset_neq_cond dest: all_lits_of_mm_diffD
+        dest: multi_member_split)
+  have 2: \<open>remove1_mset C {#Ca \<in># dom_m N. L \<in> set (watched_l (N \<propto> Ca))#} =
+     removeAll_mset C {#Ca \<in># dom_m N. L \<in> set (watched_l (N \<propto> Ca))#}\<close> for L
+    apply (rule distinct_mset_remove1_All)
+    using distinct_mset_dom[of N]
+    by (auto intro: distinct_mset_filter)
+  have [simp]: \<open>filter_mset (\<lambda>i. i \<in># remove1_mset C (dom_m N)) A  =
+    removeAll_mset C (filter_mset (\<lambda>i. i \<in># dom_m N) A)\<close> for A
+    by (induction A)
+      (auto simp: distinct_mset_remove1_All distinct_mset_dom)
+  show \<open>correct_watching'' (M, fmdrop C N, D, add_mset (mset (N \<propto> C)) NE, UE, NS, {#}, N0, U0, Q, W)\<close>
+    unfolding correct_watching''.simps clause_to_update_def
+    apply (intro conjI impI ballI)
+    subgoal for L
+      using distinct_mset_dom[of N] H1[of L \<open>fst iK\<close> \<open>fst (snd iK)\<close> \<open>snd (snd iK)\<close>] C irred
+        Hdist[of L] irred C
+      apply (auto simp: image_mset_remove1_mset_if clause_to_update_def image_filter_replicate_mset
+      distinct_mset_remove1_All filter_mset_neq_cond correctly_marked_as_binary.simps dest: all_lits_of_mm_diffD
+        dest: multi_member_split)
+      done
+    subgoal for L iK
+      using distinct_mset_dom[of N] H1[of L \<open>fst iK\<close> \<open>fst (snd iK)\<close> \<open>snd (snd iK)\<close>] C irred
+      apply (auto simp: image_mset_remove1_mset_if clause_to_update_def image_filter_replicate_mset
+      distinct_mset_remove1_All filter_mset_neq_cond correctly_marked_as_binary.simps dest: all_lits_of_mm_diffD
+        dest: multi_member_split)
+      done
+    subgoal for L
+      using C irred apply -
+      unfolding get_clauses_l.simps
+      apply (subst 1)
+      by (auto 5 1  simp: image_mset_remove1_mset_if clause_to_update_def image_filter_replicate_mset
+        distinct_mset_remove1_All filter_mset_neq_cond 2 H2 dest: all_lits_of_mm_diffD
+        dest: multi_member_split)
+    done
+  have [dest!]: \<open>x \<in># all_learned_lits_of_wl ([], N, D, NE, UE, NS, {#}, N0, U0, Q, W) \<Longrightarrow>
+           x \<in># all_learned_lits_of_wl ([], N, D, NE, UE, NS, US, N0, U0, Q, W)\<close> for x
+    using assms
+    by (auto dest: all_lits_of_mm_diffD simp: all_learned_lits_of_wl_def
+      all_lits_of_mm_union image_mset_remove1_mset_if)
+  have \<open>(N \<propto> C, irred N C) \<in># (init_clss_l N)\<close>
+    using assms by (auto simp: ran_m_def dest!: multi_member_split) (metis prod.collapse)
+  from multi_member_split[OF this]
+  show \<open>literals_are_\<L>\<^sub>i\<^sub>n' (M, fmdrop C N, D, add_mset (mset (N \<propto> C)) NE, UE, NS, {#}, N0, U0, Q, W)\<close>
+    using distinct_mset_dom[of N]
+    using assms by (auto simp: blits_in_\<L>\<^sub>i\<^sub>n'_def image_mset_remove1_mset_if all_lits_of_mm_add_mset
+          all_lits_of_mm_union literals_are_\<L>\<^sub>i\<^sub>n'_def all_init_lits_def
+       dest: multi_member_split all_lits_of_mm_diffD)
+qed
+
+
+lemma correct_watching''_fmdrop'':
+  assumes
+    irred: \<open>\<not>irred N C\<close> and
+    C: \<open>C \<in># dom_m N\<close> and
+    \<open>correct_watching'' (M', N, D, NE, UE, NS, US, N0, U0, Q, W)\<close> and
+    \<open>literals_are_\<L>\<^sub>i\<^sub>n' (M', N, D, NE, UE, NS, US, N0, U0, Q, W)\<close>
+  shows \<open>correct_watching'' (M, fmdrop C N, D, NE, add_mset (mset (N \<propto> C)) UE, NS, {#}, N0, U0, Q, W)\<close> and
+    \<open>literals_are_\<L>\<^sub>i\<^sub>n' (M, fmdrop C N, D, NE, add_mset (mset (N \<propto> C)) UE, NS, {#},  N0, U0, Q, W)\<close>
+proof -
+  let ?S = \<open>(M', N, D, NE, UE, NS, US, N0, U0, Q, W)\<close>
+  let ?\<L> = \<open>all_init_lits_of_wl ?S\<close>
+  have
+    Hdist: \<open>\<And>L. L\<in>#?\<L> \<Longrightarrow>
+       distinct_watched (W L)\<close> and
+    H1: \<open>\<And>L i K b. L\<in>#?\<L> \<Longrightarrow>
+       (i, K, b)\<in>#mset (W L) \<Longrightarrow> i \<in># dom_m N \<Longrightarrow> K \<in> set (N \<propto> i) \<and>
+          K \<noteq> L\<close> and
+    H2: \<open>\<And>L. L\<in>#?\<L> \<Longrightarrow>
+       {#i \<in># fst `# mset (W L). i \<in># dom_m N#} =
+       {#C \<in># dom_m (get_clauses_l (M', N, D, NE, UE, NS, US, N0, U0, {#}, {#})).
+        L \<in> set (watched_l (get_clauses_l (M', N, D, NE, UE, NS, US, N0, U0, {#}, {#}) \<propto> C))#}\<close>
+    using assms
+    unfolding correct_watching''.simps clause_to_update_def
+    by blast+
+  have 1: \<open>{#Ca \<in># dom_m (fmdrop C N). L \<in> set (watched_l (fmdrop C N \<propto> Ca))#} =
+    {#Ca \<in># dom_m (fmdrop C N). L \<in> set (watched_l (N \<propto> Ca))#}\<close> for L
+    apply (rule filter_mset_cong2)
+      using distinct_mset_dom[of N] H1[of L \<open>fst iK\<close> \<open>snd iK\<close>] C irred
+    by (auto simp: image_mset_remove1_mset_if clause_to_update_def image_filter_replicate_mset
+      distinct_mset_remove1_All filter_mset_neq_cond dest: all_lits_of_mm_diffD
+        dest: multi_member_split)
+  have 2: \<open>remove1_mset C {#Ca \<in># dom_m N. L \<in> set (watched_l (N \<propto> Ca))#} =
+     removeAll_mset C {#Ca \<in># dom_m N. L \<in> set (watched_l (N \<propto> Ca))#}\<close> for L
+    apply (rule distinct_mset_remove1_All)
+    using distinct_mset_dom[of N]
+    by (auto intro: distinct_mset_filter)
+  have [simp]: \<open>filter_mset (\<lambda>i. i \<in># remove1_mset C (dom_m N)) A  =
+    removeAll_mset C (filter_mset (\<lambda>i. i \<in># dom_m N) A)\<close> for A
+    by (induction A)
+      (auto simp: distinct_mset_remove1_All distinct_mset_dom)
+  show  \<open>correct_watching'' (M, fmdrop C N, D, NE, add_mset (mset (N \<propto> C)) UE, NS, {#}, N0, U0, Q, W)\<close>
+    unfolding correct_watching''.simps clause_to_update_def
+    apply (intro conjI impI ballI)
+    subgoal for L
+      using distinct_mset_dom[of N] H1[of L \<open>fst iK\<close> \<open>fst (snd iK)\<close> \<open>snd (snd iK)\<close>] C irred
+        Hdist[of L] assms
+      apply (auto simp: image_mset_remove1_mset_if clause_to_update_def image_filter_replicate_mset
+      distinct_mset_remove1_All filter_mset_neq_cond correctly_marked_as_binary.simps dest: all_lits_of_mm_diffD
+        dest: multi_member_split)
+      done
+    subgoal for L iK
+      using distinct_mset_dom[of N] H1[of L \<open>fst iK\<close> \<open>fst (snd iK)\<close> \<open>snd (snd iK)\<close>] C irred
+      apply (auto simp: image_mset_remove1_mset_if clause_to_update_def image_filter_replicate_mset
+      distinct_mset_remove1_All filter_mset_neq_cond correctly_marked_as_binary.simps dest: all_lits_of_mm_diffD
+        dest: multi_member_split)
+      done
+    subgoal for L
+      using C irred apply -
+      unfolding get_clauses_l.simps
+      apply (subst 1)
+      by (auto 5 1  simp: image_mset_remove1_mset_if clause_to_update_def image_filter_replicate_mset
+        distinct_mset_remove1_All filter_mset_neq_cond 2 H2 dest: all_lits_of_mm_diffD
+        dest: multi_member_split)
+    done
+
+  have [dest!]: \<open>x \<in># all_learned_lits_of_wl ([], N, D, NE, UE, NS, {#}, N0, U0, Q, W) \<Longrightarrow>
+           x \<in># all_learned_lits_of_wl ([], N, D, NE, UE, NS, US, N0, U0, Q, W)\<close> for x
+    using assms
+    by (auto dest: all_lits_of_mm_diffD simp: all_learned_lits_of_wl_def
+      all_lits_of_mm_union image_mset_remove1_mset_if)
+  have \<open>(N \<propto> C, irred N C) \<in># (learned_clss_l N)\<close>
+    using assms by (auto simp: ran_m_def dest!: multi_member_split) (metis prod.collapse)
+  from multi_member_split[OF this]
+  show \<open>literals_are_\<L>\<^sub>i\<^sub>n' (M, fmdrop C N, D, NE, add_mset (mset (N \<propto> C)) UE, NS, {#}, N0, U0, Q, W)\<close>
+    using distinct_mset_dom[of N]
+    using assms by (auto simp: blits_in_\<L>\<^sub>i\<^sub>n'_def image_mset_remove1_mset_if all_lits_of_mm_add_mset
+          all_lits_of_mm_union literals_are_\<L>\<^sub>i\<^sub>n'_def all_init_lits_def
+       dest: multi_member_split all_lits_of_mm_diffD)
+qed
+
+definition remove_one_annot_true_clause_one_imp_wl_pre where
+  \<open>remove_one_annot_true_clause_one_imp_wl_pre i T \<longleftrightarrow>
+     (\<exists>T'. (T, T') \<in> state_wl_l None \<and>
+       remove_one_annot_true_clause_one_imp_pre i T' \<and>
+       correct_watching'' T \<and> literals_are_\<L>\<^sub>i\<^sub>n' T)\<close>
+
+definition replace_annot_wl_pre :: \<open>'v literal \<Rightarrow> nat \<Rightarrow> 'v twl_st_wl \<Rightarrow> bool\<close> where
+\<open>replace_annot_wl_pre L C S \<longleftrightarrow>
+  (\<exists>S'. (S, S') \<in> state_wl_l None \<and> L \<in># all_init_lits_of_wl S \<and>
+    replace_annot_l_pre L C S' \<and> literals_are_\<L>\<^sub>i\<^sub>n' S \<and>
+    correct_watching'' S)\<close>
+
+definition replace_annot_wl :: \<open>'v literal \<Rightarrow> nat \<Rightarrow> 'v twl_st_wl \<Rightarrow> 'v twl_st_wl nres\<close> where
+  \<open>replace_annot_wl L C =
+    (\<lambda>(M, N, D, NE, UE, NS, US, N0, U0, Q, W). do {
+      ASSERT(replace_annot_wl_pre L C (M, N, D, NE, UE, NS, US, N0, U0, Q, W));
+      RES {(M', N, D, NE, UE, NS, {#}, N0, U0, Q, W)| M'.
+       (\<exists>M2 M1 C. M = M2 @ Propagated L C # M1 \<and> M' = M2 @ Propagated L 0 # M1)}
+   })\<close>
+
+lemma replace_annot_l_pre_replace_annot_wl_pre: \<open>(((L, C), S), (L', C'), S')
+    \<in> Id \<times>\<^sub>f nat_rel \<times>\<^sub>f
+      {(S, T).
+       (S, T) \<in> state_wl_l None \<and>
+       correct_watching'' S \<and> literals_are_\<L>\<^sub>i\<^sub>n' S} \<Longrightarrow>
+    replace_annot_l_pre L' C' S' \<Longrightarrow>
+    replace_annot_wl_pre L C S\<close>
+    unfolding replace_annot_wl_pre_def replace_annot_l_pre_alt_def
+    unfolding replace_annot_l_pre_def[symmetric]
+    by (rule exI[of _ \<open>S'\<close>])
+      (auto simp add: ac_simps all_init_lits_of_wl_def)
+
+lemma all_learned_lits_of_wl_all_init_lits_of_wlD[intro]:
+  \<open>set_mset (all_learned_lits_of_wl (M, ab, ac, ad, ae, af, ag, ah, ai, aj, ba))
+       \<subseteq> set_mset (all_init_lits_of_wl (M, ab, ac, ad, ae, af, {#}, ah, ai, aj, ba)) \<Longrightarrow>
+       x \<in># all_learned_lits_of_wl (M, ab, ac, ad, ae, af, {#}, ah, ai, aj, ba) \<Longrightarrow>
+       x \<in># all_init_lits_of_wl (M, ab, ac, ad, ae, af, {#}, ah, ai, aj, ba)\<close>
+  by (auto simp: all_learned_lits_of_wl_def all_init_lits_of_wl_def
+    all_lits_of_mm_union)
+
+lemma replace_annot_wl_replace_annot_l:
+  \<open>(uncurry2 replace_annot_wl, uncurry2 replace_annot_l) \<in>
+    Id \<times>\<^sub>f nat_rel \<times>\<^sub>f {(S, T). (S, T) \<in> state_wl_l None \<and> correct_watching'' S \<and>
+        literals_are_\<L>\<^sub>i\<^sub>n' S} \<rightarrow>\<^sub>f
+    \<langle>{(S, T). (S, T) \<in> state_wl_l None \<and> correct_watching'' S \<and>
+        literals_are_\<L>\<^sub>i\<^sub>n' S}\<rangle>nres_rel\<close>
+    unfolding replace_annot_wl_def replace_annot_l_def uncurry_def
+    apply (intro frefI nres_relI)
+    apply clarify
+    apply refine_rcg
+    subgoal for a b aa ab ac ad ae af ba ag bb ah ai aj ak al am bc
+      by (force intro!: replace_annot_l_pre_replace_annot_wl_pre)
+    subgoal
+      by (rule RES_refine)
+        (force simp: state_wl_l_def literals_are_\<L>\<^sub>i\<^sub>n'_def ac_simps
+          all_lits_of_mm_union
+          correct_watching''.simps clause_to_update_def blits_in_\<L>\<^sub>i\<^sub>n'_def)
+    done
+
+definition remove_and_add_cls_wl :: \<open>nat \<Rightarrow> 'v twl_st_wl \<Rightarrow> 'v twl_st_wl nres\<close> where
+  \<open>remove_and_add_cls_wl C =
+    (\<lambda>(M, N, D, NE, UE, NS, US, Q, W). do {
+       ASSERT(C \<in># dom_m N);
+        RETURN (M, fmdrop C N, D,
+         (if irred N C then add_mset (mset (N\<propto>C)) else id) NE,
+	 (if \<not>irred N C then add_mset (mset (N\<propto>C)) else id) UE, NS, {#}, Q, W)
+    })\<close>
+
+definition remove_one_annot_true_clause_one_imp_wl
+  :: \<open>nat \<Rightarrow> 'v twl_st_wl \<Rightarrow> (nat \<times> 'v twl_st_wl) nres\<close>
+where
+\<open>remove_one_annot_true_clause_one_imp_wl = (\<lambda>i S. do {
+      ASSERT(remove_one_annot_true_clause_one_imp_wl_pre i S);
+      ASSERT(is_proped (rev (get_trail_wl S) ! i));
+      (L, C) \<leftarrow> SPEC(\<lambda>(L, C). (rev (get_trail_wl S))!i = Propagated L C);
+      ASSERT(Propagated L C \<in> set (get_trail_wl S));
+      ASSERT(L \<in># all_init_lits_of_wl S);
+      if C = 0 then RETURN (i+1, S)
+      else do {
+        ASSERT(C \<in># dom_m (get_clauses_wl S));
+	S \<leftarrow> replace_annot_wl L C S;
+	S \<leftarrow> remove_and_add_cls_wl C S;
+        \<comment> \<open>\<^text>\<open>S \<leftarrow> remove_all_annot_true_clause_imp_wl L S;\<close>\<close>
+        RETURN (i+1, S)
+      }
+  })\<close>
+
+lemma
+  assumes
+      x2_T: \<open>(x2, T) \<in> state_wl_l b\<close> and
+      struct: \<open>twl_struct_invs U\<close> and
+      T_U: \<open>(T, U) \<in> twl_st_l b'\<close>
+  shows
+    literals_are_\<L>\<^sub>i\<^sub>n_literals_are_\<L>\<^sub>i\<^sub>n_trail_init:
+      \<open>literals_are_in_\<L>\<^sub>i\<^sub>n_trail (all_init_atms_st x2) (get_trail_wl x2)\<close>
+     (is \<open>?trail\<close>)
+proof -
+  have
+    alien: \<open>cdcl\<^sub>W_restart_mset.no_strange_atm (state\<^sub>W_of U)\<close> and
+    confl: \<open>cdcl\<^sub>W_restart_mset.cdcl\<^sub>W_conflicting (state\<^sub>W_of U)\<close> and
+    M_lev: \<open>cdcl\<^sub>W_restart_mset.cdcl\<^sub>W_M_level_inv (state\<^sub>W_of U)\<close> and
+    dist: \<open>cdcl\<^sub>W_restart_mset.distinct_cdcl\<^sub>W_state (state\<^sub>W_of U)\<close>
+   using struct unfolding twl_struct_invs_def cdcl\<^sub>W_restart_mset.cdcl\<^sub>W_all_struct_inv_def
+        pcdcl_all_struct_invs_def state\<^sub>W_of_def
+   by fast+
+
+  show lits_trail: \<open>literals_are_in_\<L>\<^sub>i\<^sub>n_trail (all_init_atms_st x2) (get_trail_wl x2)\<close>
+    using alien x2_T T_U unfolding is_\<L>\<^sub>a\<^sub>l\<^sub>l_def
+      literals_are_in_\<L>\<^sub>i\<^sub>n_trail_def cdcl\<^sub>W_restart_mset.no_strange_atm_def
+      literals_are_\<L>\<^sub>i\<^sub>n_def all_init_lits_of_wl_def all_atms_def \<L>\<^sub>a\<^sub>l\<^sub>l_all_init_atms
+    by
+     (auto 5 2
+        simp del: all_clss_l_ran_m union_filter_mset_complement
+        simp: twl_st twl_st_l twl_st_wl all_lits_of_mm_union lits_of_def
+        convert_lits_l_def image_image in_all_lits_of_mm_ain_atms_of_iff
+        get_unit_clauses_wl_alt_def \<L>\<^sub>a\<^sub>l\<^sub>l_all_init_atms all_init_lits_def)
+qed
+
+lemma remove_one_annot_true_clause_one_imp_wl_remove_one_annot_true_clause_one_imp:
+    \<open>(uncurry remove_one_annot_true_clause_one_imp_wl, uncurry remove_one_annot_true_clause_one_imp)
+    \<in> nat_rel \<times>\<^sub>f  {(S, T). (S, T) \<in> state_wl_l None \<and> correct_watching'' S \<and> literals_are_\<L>\<^sub>i\<^sub>n' S} \<rightarrow>\<^sub>f
+      \<langle>nat_rel \<times>\<^sub>f {(S, T). (S, T) \<in> state_wl_l None \<and> correct_watching'' S \<and> literals_are_\<L>\<^sub>i\<^sub>n' S}\<rangle>nres_rel\<close>
+    (is \<open>_ \<in> _ \<times>\<^sub>f ?A \<rightarrow>\<^sub>f _\<close>)
+proof -
+
+  have [refine0]: \<open>remove_and_add_cls_wl C S \<le>\<Down> ?A (remove_and_add_cls_l C' S')\<close>
+    if \<open>(C, C') \<in> Id\<close> and \<open>(S, S') \<in> ?A\<close>
+      for C C' S S'
+    using that unfolding remove_and_add_cls_l_def remove_and_add_cls_wl_def
+    by refine_rcg
+     (auto intro!: RES_refine simp: state_wl_l_def
+       intro: correct_watching''_fmdrop correct_watching''_fmdrop''
+          correct_watching''_fmdrop')
+
+  show ?thesis
+    unfolding remove_one_annot_true_clause_one_imp_wl_def remove_one_annot_true_clause_one_imp_def
+      uncurry_def
+    apply (intro frefI nres_relI)
+    apply (refine_vcg replace_annot_wl_replace_annot_l[THEN fref_to_Down_curry2])
+    subgoal for x y unfolding remove_one_annot_true_clause_one_imp_wl_pre_def
+      by (rule exI[of _ \<open>snd y\<close>]) auto
+    subgoal by (simp add: state_wl_l_def)
+    subgoal by (simp add: state_wl_l_def)
+    subgoal by (simp add: state_wl_l_def)
+    subgoal for x y x1 x2 x1a x2a xa x' x1b x2b x1c x2c
+      unfolding remove_one_annot_true_clause_one_imp_wl_pre_def
+       remove_one_annot_true_clause_one_imp_pre_def
+      apply normalize_goal+
+
+      subgoal for U S T
+        using literals_are_\<L>\<^sub>i\<^sub>n_literals_are_\<L>\<^sub>i\<^sub>n_trail_init[of x2a U None T None]
+        by (auto simp add: literals_are_in_\<L>\<^sub>i\<^sub>n_trail_def lits_of_def image_image
+          \<L>\<^sub>a\<^sub>l\<^sub>l_all_init_atms)
+       done
+    subgoal by simp
+    subgoal by (simp add: state_wl_l_def)
+    subgoal by (simp add: state_wl_l_def)
+    subgoal by (simp add: state_wl_l_def)
+    subgoal by simp
+    subgoal by (simp add: state_wl_l_def)
+    done
+qed
+
+definition remove_one_annot_true_clause_imp_wl_inv where
+  \<open>remove_one_annot_true_clause_imp_wl_inv S = (\<lambda>(i, T).
+     (\<exists>S' T'. (S, S') \<in> state_wl_l None \<and> (T, T') \<in> state_wl_l None \<and>
+       correct_watching'' S \<and> correct_watching'' T \<and> literals_are_\<L>\<^sub>i\<^sub>n' S \<and>
+       literals_are_\<L>\<^sub>i\<^sub>n' T \<and>
+       remove_one_annot_true_clause_imp_inv S' (i, T')))\<close>
+
+definition remove_all_learned_subsumed_clauses_wl :: \<open>'v twl_st_wl \<Rightarrow> ('v twl_st_wl) nres\<close> where
+\<open>remove_all_learned_subsumed_clauses_wl = (\<lambda>(M, N, D, NE, UE, NS, US, N0, U0, Q, W).
+   RETURN (M, N, D, NE, UE, NS, {#}, N0, U0, Q, W))\<close>
+
+definition remove_one_annot_true_clause_imp_wl :: \<open>'v twl_st_wl \<Rightarrow> ('v twl_st_wl) nres\<close>
+where
+\<open>remove_one_annot_true_clause_imp_wl = (\<lambda>S. do {
+    k \<leftarrow> SPEC(\<lambda>k. (\<exists>M1 M2 K. (Decided K # M1, M2) \<in> set (get_all_ann_decomposition (get_trail_wl S)) \<and>
+        count_decided M1 = 0 \<and> k = length M1)
+      \<or> (count_decided (get_trail_wl S) = 0 \<and> k = length (get_trail_wl S)));
+    (_, S) \<leftarrow> WHILE\<^sub>T\<^bsup>remove_one_annot_true_clause_imp_wl_inv S\<^esup>
+      (\<lambda>(i, S). i < k)
+      (\<lambda>(i, S). remove_one_annot_true_clause_one_imp_wl i S)
+      (0, S);
+    remove_all_learned_subsumed_clauses_wl S
+  })\<close>
+
+lemma remove_all_learned_subsumed_clauses_wl_remove_all_learned_subsumed_clauses:
+  \<open>(remove_all_learned_subsumed_clauses_wl, remove_all_learned_subsumed_clauses)
+   \<in> {(S, T). (S, T) \<in> state_wl_l None \<and> correct_watching'' S \<and> literals_are_\<L>\<^sub>i\<^sub>n' S} \<rightarrow>\<^sub>f
+      \<langle>{(S, T). (S, T) \<in> state_wl_l None \<and> correct_watching'' S \<and> literals_are_\<L>\<^sub>i\<^sub>n' S}\<rangle>nres_rel\<close>
+  by (force intro!: frefI nres_relI
+    simp: remove_all_learned_subsumed_clauses_wl_def remove_all_learned_subsumed_clauses_def
+      literals_are_\<L>\<^sub>i\<^sub>n'_def correct_watching''.simps state_wl_l_def
+      clause_to_update_def all_lits_of_mm_union blits_in_\<L>\<^sub>i\<^sub>n'_def)
+
+lemma remove_one_annot_true_clause_imp_wl_remove_one_annot_true_clause_imp:
+  \<open>(remove_one_annot_true_clause_imp_wl, remove_one_annot_true_clause_imp)
+    \<in> {(S, T). (S, T) \<in> state_wl_l None \<and> correct_watching'' S \<and> literals_are_\<L>\<^sub>i\<^sub>n' S} \<rightarrow>\<^sub>f
+      \<langle>{(S, T). (S, T) \<in> state_wl_l None \<and> correct_watching'' S \<and> literals_are_\<L>\<^sub>i\<^sub>n' S}\<rangle>nres_rel\<close>
+proof -
+  show ?thesis
+    unfolding remove_one_annot_true_clause_imp_wl_def remove_one_annot_true_clause_imp_def
+      uncurry_def
+    apply (intro frefI nres_relI)
+    apply (refine_vcg
+      WHILEIT_refine[where
+         R = \<open>nat_rel \<times>\<^sub>f {(S, T).  (S, T) \<in> state_wl_l None \<and> correct_watching'' S \<and>
+            literals_are_\<L>\<^sub>i\<^sub>n' S}\<close>]
+      remove_one_annot_true_clause_one_imp_wl_remove_one_annot_true_clause_one_imp[THEN
+        fref_to_Down_curry]
+      remove_all_learned_subsumed_clauses_wl_remove_all_learned_subsumed_clauses[THEN
+        fref_to_Down])
+    subgoal by force
+    subgoal by auto
+    subgoal for x y k ka xa x'
+      unfolding remove_one_annot_true_clause_imp_wl_inv_def
+      apply (subst case_prod_beta)
+      apply (rule_tac x=\<open>y\<close> in exI)
+      apply (rule_tac x=\<open>snd x'\<close> in exI)
+      apply (subst (asm)(18) surjective_pairing)
+      apply (subst (asm)(23) surjective_pairing)
+      unfolding prod_rel_iff by simp
+    subgoal by auto
+    subgoal by auto
+    subgoal by auto
+    done
+qed
+
+definition collect_valid_indices_wl :: \<open>'v twl_st_wl \<Rightarrow> nat list nres\<close> where
+  \<open>collect_valid_indices_wl S = SPEC (\<lambda>N. True)\<close>
+
+definition mark_to_delete_clauses_wl_inv
+  :: \<open>'v twl_st_wl \<Rightarrow> nat list \<Rightarrow> nat \<times> 'v twl_st_wl\<times> nat list  \<Rightarrow> bool\<close>
+where
+  \<open>mark_to_delete_clauses_wl_inv = (\<lambda>S xs0 (i, T, xs).
+     \<exists>S' T'. (S, S') \<in> state_wl_l None \<and> (T, T') \<in> state_wl_l None \<and>
+      mark_to_delete_clauses_l_inv S' xs0 (i, T', xs) \<and>
+      correct_watching' S\<and> literals_are_\<L>\<^sub>i\<^sub>n' S \<and> literals_are_\<L>\<^sub>i\<^sub>n' T)\<close>
+
+definition mark_to_delete_clauses_wl_pre :: \<open>'v twl_st_wl \<Rightarrow> bool\<close>
+where
+  \<open>mark_to_delete_clauses_wl_pre S \<longleftrightarrow>
+   (\<exists>T. (S, T) \<in> state_wl_l None \<and> mark_to_delete_clauses_l_pre T \<and> literals_are_\<L>\<^sub>i\<^sub>n' S)\<close>
+
+definition mark_garbage_wl:: \<open>nat \<Rightarrow> 'v twl_st_wl \<Rightarrow> 'v twl_st_wl\<close>  where
+  \<open>mark_garbage_wl = (\<lambda>C (M, N, D, NE, UE, NS, US, N0, U0, WS, Q).
+    (M, fmdrop C N, D, NE, UE, NS, {#}, N0, U0, WS, Q))\<close>
+
+definition mark_to_delete_clauses_wl :: \<open>'v twl_st_wl \<Rightarrow> 'v twl_st_wl nres\<close> where
+\<open>mark_to_delete_clauses_wl  = (\<lambda>S. do {
+    ASSERT(mark_to_delete_clauses_wl_pre S);
+    xs \<leftarrow> collect_valid_indices_wl S;
+    l \<leftarrow> SPEC(\<lambda>_:: nat. True);
+    (_, S, _) \<leftarrow> WHILE\<^sub>T\<^bsup>mark_to_delete_clauses_wl_inv S xs\<^esup>
+      (\<lambda>(i, S, xs). i < length xs)
+      (\<lambda>(i, T, xs). do {
+        if(xs!i \<notin># dom_m (get_clauses_wl T)) then RETURN (i, T, delete_index_and_swap xs i)
+        else do {
+          ASSERT(0 < length (get_clauses_wl T\<propto>(xs!i)));
+	  ASSERT (get_clauses_wl T \<propto> (xs ! i) ! 0 \<in># \<L>\<^sub>a\<^sub>l\<^sub>l (all_init_atms_st T));
+          can_del \<leftarrow> SPEC(\<lambda>b. b \<longrightarrow>
+             (Propagated (get_clauses_wl T\<propto>(xs!i)!0) (xs!i) \<notin> set (get_trail_wl T)) \<and>
+              \<not>irred (get_clauses_wl T) (xs!i) \<and> length (get_clauses_wl T \<propto> (xs!i)) \<noteq> 2);
+          ASSERT(i < length xs);
+          if can_del
+          then
+            RETURN (i, mark_garbage_wl (xs!i) T, delete_index_and_swap xs i)
+          else
+            RETURN (i+1, T, xs)
+       }
+      })
+      (l, S, xs);
+    remove_all_learned_subsumed_clauses_wl S
+  })\<close>
+
+lemma mark_to_delete_clauses_wl_invD1:
+  assumes \<open>mark_to_delete_clauses_wl_inv S xs (i, T, ys)\<close> and
+    \<open>C \<in># dom_m (get_clauses_wl T)\<close> and
+    \<open>0 < length (get_clauses_wl T \<propto> C)\<close>
+  shows
+    \<open>get_clauses_wl T \<propto> C ! 0 \<in># \<L>\<^sub>a\<^sub>l\<^sub>l (all_init_atms_st T)\<close>
+proof -
+  have \<open>literals_are_\<L>\<^sub>i\<^sub>n' T\<close>
+    using assms unfolding mark_to_delete_clauses_wl_inv_def by blast
+  then have \<open>get_clauses_wl T \<propto> C ! 0 \<in># all_init_lits_of_wl T\<close>
+    using nth_in_all_lits_stI[of C T 0]
+    using assms(2,3) by (auto simp del: nth_in_all_lits_stI
+      simp: all_lits_st_init_learned  literals_are_\<L>\<^sub>i\<^sub>n'_def)
+  then show \<open>?thesis\<close>
+    by (simp add: \<L>\<^sub>a\<^sub>l\<^sub>l_all_init_atms)
+qed
+
+lemma remove_all_learned_subsumed_clauses_wl_remove_all_learned_subsumed_clauses2:
+  \<open>(remove_all_learned_subsumed_clauses_wl, remove_all_learned_subsumed_clauses)
+   \<in> {(S, T). (S, T) \<in> state_wl_l None \<and> correct_watching' S \<and> literals_are_\<L>\<^sub>i\<^sub>n' S} \<rightarrow>\<^sub>f
+      \<langle>{(S, T). (S, T) \<in> state_wl_l None \<and> correct_watching' S \<and> literals_are_\<L>\<^sub>i\<^sub>n' S}\<rangle>nres_rel\<close>
+  by (force intro!: frefI nres_relI
+    simp: remove_all_learned_subsumed_clauses_wl_def remove_all_learned_subsumed_clauses_def
+      literals_are_\<L>\<^sub>i\<^sub>n'_def correct_watching'.simps state_wl_l_def
+      clause_to_update_def all_lits_of_mm_union blits_in_\<L>\<^sub>i\<^sub>n'_def)
+
+lemma mark_to_delete_clauses_wl_mark_to_delete_clauses_l:
+  \<open>(mark_to_delete_clauses_wl, mark_to_delete_clauses_l)
+    \<in> {(S, T). (S, T) \<in> state_wl_l None \<and> correct_watching' S \<and> literals_are_\<L>\<^sub>i\<^sub>n' S} \<rightarrow>\<^sub>f
+      \<langle>{(S, T). (S, T) \<in> state_wl_l None \<and> correct_watching' S \<and> literals_are_\<L>\<^sub>i\<^sub>n' S}\<rangle>nres_rel\<close>
+proof -
+  have [refine0]: \<open>collect_valid_indices_wl S  \<le> \<Down> Id  (collect_valid_indices S')\<close>
+    if \<open>(S, S') \<in> {(S, T).  (S, T) \<in> state_wl_l None \<and> correct_watching' S \<and>
+           mark_to_delete_clauses_wl_pre S}\<close>
+    for S S'
+    using that by (auto simp: collect_valid_indices_wl_def collect_valid_indices_def)
+  have if_inv: \<open>(if A then RETURN P else RETURN Q) = RETURN (if A then P else Q)\<close> for A P Q
+    by auto
+  have Ball_range[simp]: \<open>(\<forall>x\<in>range f \<union> range g. P x)\<longleftrightarrow>(\<forall>x. P (f x) \<and> P (g x))\<close> for P f g
+    by auto
+  show ?thesis
+    unfolding mark_to_delete_clauses_wl_def mark_to_delete_clauses_l_def
+      uncurry_def
+    apply (intro frefI nres_relI)
+    apply (refine_vcg
+      WHILEIT_refine[where
+         R = \<open>{((i, S, xs), (j, T, ys)). i = j \<and> (S, T) \<in> state_wl_l None \<and> correct_watching' S \<and>
+             xs = ys \<and> literals_are_\<L>\<^sub>i\<^sub>n' S}\<close>]
+      remove_one_annot_true_clause_one_imp_wl_remove_one_annot_true_clause_one_imp[THEN
+        fref_to_Down_curry]
+      remove_all_learned_subsumed_clauses_wl_remove_all_learned_subsumed_clauses2[THEN
+        fref_to_Down])
+    subgoal unfolding mark_to_delete_clauses_wl_pre_def by blast
+    subgoal by auto
+    subgoal by (auto simp: state_wl_l_def)
+    subgoal unfolding mark_to_delete_clauses_wl_inv_def by fast
+    subgoal by auto
+    subgoal by (force simp: state_wl_l_def)
+    subgoal by auto
+    subgoal by (force simp: state_wl_l_def)
+    subgoal for x y xs xsa l to_keep xa x' x1 x2 x1a x2a x1b x2b x1c x2c
+      by (auto simp: mark_to_delete_clauses_wl_invD1)
+    subgoal by (auto simp: state_wl_l_def can_delete_def)
+    subgoal by auto
+    subgoal by (force simp: state_wl_l_def)
+    subgoal
+      by (auto simp: state_wl_l_def correct_watching_fmdrop mark_garbage_wl_def
+          mark_garbage_l_def ac_simps
+        split: prod.splits)
+    subgoal by (auto simp: state_wl_l_def)
+    subgoal by (auto simp: state_wl_l_def)
+    done
+qed
+
+text \<open>
+  This is only a specification and must be implemented. There are two ways to do so:
+  \<^enum> clean the watch lists and then iterate over all clauses to rebuild them.
+  \<^enum> iterate over the watch list and check whether the clause index is in the domain or not.
+
+  It is not clear which is faster (but option 1 requires only 1 memory access per clause instead of
+  two). The first option is implemented in SPASS-SAT. The latter version (partly) in cadical.
+\<close>
+definition rewatch_clauses :: \<open>'v twl_st_wl \<Rightarrow> 'v twl_st_wl nres\<close> where
+  \<open>rewatch_clauses = (\<lambda>(M, N, D, NE, UE, NS, US, N0, U0, Q, W).
+  SPEC(\<lambda>(M', N', D', NE', UE', NS', US', N0', U0', Q', W').
+     (M, N, D, NE, UE, NS, US, N0, U0, Q) = (M', N', D', NE', UE', NS', US', N0', U0', Q') \<and>
+    correct_watching (M, N', D, NE, UE, NS', US', N0', U0', Q, W')))\<close>
+
+definition mark_to_delete_clauses_wl_post where
+  \<open>mark_to_delete_clauses_wl_post S T \<longleftrightarrow>
+     (\<exists>S' T'. (S, S') \<in> state_wl_l None \<and> (T, T') \<in> state_wl_l None \<and> blits_in_\<L>\<^sub>i\<^sub>n S \<and>
+       mark_to_delete_clauses_l_post S' T' \<and> correct_watching S \<and> blits_in_\<L>\<^sub>i\<^sub>n T \<and>
+       correct_watching T)\<close>
+
+definition cdcl_twl_full_restart_wl_prog :: \<open>'v twl_st_wl \<Rightarrow> 'v twl_st_wl nres\<close> where
+\<open>cdcl_twl_full_restart_wl_prog S = do {
+    \<comment> \<open> \<^term>\<open>remove_one_annot_true_clause_imp_wl S\<close>\<close>
+    ASSERT(mark_to_delete_clauses_wl_pre S);
+    T \<leftarrow> mark_to_delete_clauses_wl S;
+    ASSERT(mark_to_delete_clauses_wl_post S T);
+    RETURN T
+  }\<close>
+
+
+lemma correct_watching_correct_watching: \<open>correct_watching S \<Longrightarrow> correct_watching' S\<close>
+  by (cases S, auto simp only: correct_watching.simps correct_watching'.simps all_lits_st_init_learned
+    image_mset_union)
+
+lemma (in -) [twl_st_l, simp]:
+ \<open>(Sa, x) \<in> twl_st_l None \<Longrightarrow> get_all_learned_clss x =  mset `# (get_learned_clss_l Sa) + get_unit_learned_clss_l Sa + get_subsumed_learned_clauses_l Sa + get_learned_clauses0_l Sa\<close>
+  by (cases Sa; cases x) (auto simp: twl_st_l_def get_learned_clss_l_def mset_take_mset_drop_mset')
+
+lemma cdcl_twl_full_restart_wl_prog_final_rel:
+  assumes
+    S_Sa: \<open>(S, Sa) \<in> {(S, T). (S, T) \<in> state_wl_l None \<and> correct_watching' S \<and> blits_in_\<L>\<^sub>i\<^sub>n S}\<close> and
+    pre_Sa: \<open>mark_to_delete_clauses_l_pre Sa\<close> and
+    pre_S: \<open>mark_to_delete_clauses_wl_pre S\<close> and
+    T_Ta: \<open>(T, Ta) \<in> {(S, T). (S, T) \<in> state_wl_l None \<and> correct_watching' S \<and> literals_are_\<L>\<^sub>i\<^sub>n' S}\<close> and
+    pre_l: \<open>mark_to_delete_clauses_l_post Sa Ta\<close>
+  shows \<open>mark_to_delete_clauses_wl_post S T\<close>
+proof -
+  obtain x where
+    Sa_x: \<open>(Sa, x) \<in> twl_st_l None\<close> and
+    st: \<open>remove_one_annot_true_clause\<^sup>*\<^sup>* Sa Ta\<close> and
+    list_invs: \<open>twl_list_invs Sa\<close> and
+    struct: \<open>twl_struct_invs x\<close> and
+    confl: \<open>get_conflict_l Sa = None\<close> and
+    upd: \<open>clauses_to_update_l Sa = {#}\<close>
+    using pre_l
+    unfolding mark_to_delete_clauses_l_post_def by blast
+
+  have corr_S: \<open>correct_watching' S\<close> and corr_T: \<open>correct_watching' T\<close> and
+    blits_S: \<open>blits_in_\<L>\<^sub>i\<^sub>n S\<close> and
+    blits_T: \<open>literals_are_\<L>\<^sub>i\<^sub>n' T\<close> and
+    S_Sa: \<open>(S, Sa) \<in> state_wl_l None\<close> and
+    T_Ta: \<open>(T, Ta) \<in> state_wl_l None\<close>
+    using S_Sa T_Ta by auto
+
+  have \<open>set_mset (all_init_lits_of_wl S) = set_mset (all_lits_st S)\<close>
+    using literals_are_\<L>\<^sub>i\<^sub>n'_literals_are_\<L>\<^sub>i\<^sub>n_iff(4)[OF S_Sa Sa_x struct] .
+
+  then have corr_S': \<open>correct_watching S\<close>
+    using corr_S
+    by (cases S; simp only: correct_watching'.simps correct_watching.simps)
+  obtain y where
+    \<open>cdcl_twl_restart_l\<^sup>*\<^sup>* Sa Ta\<close> and
+    Ta_y: \<open>(Ta, y) \<in> twl_st_l None\<close>  and
+    \<open>cdcl_twl_restart\<^sup>*\<^sup>* x y\<close> and
+    struct: \<open>twl_struct_invs y\<close>
+    using rtranclp_remove_one_annot_true_clause_cdcl_twl_restart_l2[OF st list_invs confl upd Sa_x
+      struct]
+    by blast
+
+  have eq: \<open>set_mset (all_init_lits_of_wl T) = set_mset (all_lits_st T)\<close>
+    using literals_are_\<L>\<^sub>i\<^sub>n'_literals_are_\<L>\<^sub>i\<^sub>n_iff(4)[OF T_Ta Ta_y struct] .
+
+  then have corr_T': \<open>correct_watching T\<close>
+    using corr_T
+    by (cases T; simp only: correct_watching'.simps correct_watching.simps)
+
+  have \<open>blits_in_\<L>\<^sub>i\<^sub>n T\<close>
+    using blits_T eq
+    unfolding blits_in_\<L>\<^sub>i\<^sub>n_def blits_in_\<L>\<^sub>i\<^sub>n'_def all_lits_def literals_are_\<L>\<^sub>i\<^sub>n'_def
+       all_init_lits_def
+    by (auto dest: multi_member_split simp: ac_simps)
+  then show ?thesis
+    using S_Sa T_Ta corr_T' corr_S' pre_l blits_S
+    unfolding mark_to_delete_clauses_wl_post_def
+    by blast
+qed
+
+lemma cdcl_twl_full_restart_wl_prog_final_rel':
+  assumes
+    S_Sa: \<open>(S, Sa) \<in> {(S, T). (S, T) \<in> state_wl_l None \<and> correct_watching S \<and> blits_in_\<L>\<^sub>i\<^sub>n S}\<close> and
+    pre_Sa: \<open>mark_to_delete_clauses_l_pre Sa\<close> and
+    pre_S: \<open>mark_to_delete_clauses_wl_pre S\<close> and
+    T_Ta: \<open>(T, Ta) \<in> {(S, T). (S, T) \<in> state_wl_l None \<and> correct_watching' S \<and> literals_are_\<L>\<^sub>i\<^sub>n' S}\<close> and
+    pre_l: \<open>mark_to_delete_clauses_l_post Sa Ta\<close>
+  shows \<open>mark_to_delete_clauses_wl_post S T\<close>
+proof -
+  obtain x where
+    Sa_x: \<open>(Sa, x) \<in> twl_st_l None\<close> and
+    st: \<open>remove_one_annot_true_clause\<^sup>*\<^sup>* Sa Ta\<close> and
+    list_invs: \<open>twl_list_invs Sa\<close> and
+    struct: \<open>twl_struct_invs x\<close> and
+    confl: \<open>get_conflict_l Sa = None\<close> and
+    upd: \<open>clauses_to_update_l Sa = {#}\<close>
+    using pre_l
+    unfolding mark_to_delete_clauses_l_post_def by blast
+
+  have corr_S: \<open>correct_watching S\<close> and corr_T: \<open>correct_watching' T\<close> and
+    blits_T: \<open>literals_are_\<L>\<^sub>i\<^sub>n' T\<close> and
+    blits_S: \<open>blits_in_\<L>\<^sub>i\<^sub>n S\<close> and
+    S_Sa: \<open>(S, Sa) \<in> state_wl_l None\<close> and
+    T_Ta: \<open>(T, Ta) \<in> state_wl_l None\<close>
+    using S_Sa T_Ta by auto
+  have corr_S: \<open>correct_watching' S\<close>
+    using correct_watching_correct_watching[OF corr_S] .
+  have \<open>set_mset (all_init_lits_of_wl S) = set_mset (all_lits_st S)\<close>
+    using literals_are_\<L>\<^sub>i\<^sub>n'_literals_are_\<L>\<^sub>i\<^sub>n_iff(4)[OF S_Sa Sa_x struct] .
+  then have corr_S': \<open>correct_watching S\<close>
+    using corr_S
+    by (cases S; simp only: correct_watching'.simps correct_watching.simps)
+  obtain y where
+    \<open>cdcl_twl_restart_l\<^sup>*\<^sup>* Sa Ta\<close> and
+    Ta_y: \<open>(Ta, y) \<in> twl_st_l None\<close>  and
+    \<open>cdcl_twl_restart\<^sup>*\<^sup>* x y\<close> and
+    struct: \<open>twl_struct_invs y\<close>
+    using rtranclp_remove_one_annot_true_clause_cdcl_twl_restart_l2[OF st list_invs confl upd Sa_x
+      struct]
+    by blast
+
+
+  have eq: \<open>set_mset (all_init_lits_of_wl T) = set_mset (all_lits_st T)\<close>
+    using literals_are_\<L>\<^sub>i\<^sub>n'_literals_are_\<L>\<^sub>i\<^sub>n_iff(4)[OF T_Ta Ta_y struct] .
+
+  then have corr_T': \<open>correct_watching T\<close>
+    using corr_T
+    by (cases T; simp only: correct_watching'.simps correct_watching.simps)
+
+  have \<open>blits_in_\<L>\<^sub>i\<^sub>n T\<close>
+    using blits_T eq
+    unfolding blits_in_\<L>\<^sub>i\<^sub>n_def blits_in_\<L>\<^sub>i\<^sub>n'_def all_lits_def literals_are_\<L>\<^sub>i\<^sub>n'_def
+         all_init_lits_def
+    by (auto dest: multi_member_split simp: ac_simps)
+  then show ?thesis
+    using S_Sa T_Ta corr_T' corr_S' pre_l blits_S
+    unfolding mark_to_delete_clauses_wl_post_def
+    by blast
+qed
+
+
+lemma mark_to_delete_clauses_l_pre_blits_in_\<L>\<^sub>i\<^sub>n':
+  assumes
+    S_Sa: \<open>(S, Sa) \<in> {(S, T). (S, T) \<in> state_wl_l None \<and> correct_watching S \<and> blits_in_\<L>\<^sub>i\<^sub>n S}\<close> and
+    pre_Sa: \<open>mark_to_delete_clauses_l_pre Sa\<close>
+  shows \<open>literals_are_\<L>\<^sub>i\<^sub>n' S\<close>
+proof -
+  obtain x where
+    Sa_x: \<open>(Sa, x) \<in> twl_st_l None\<close> and
+    list_invs: \<open>twl_list_invs Sa\<close> and
+    struct: \<open>twl_struct_invs x\<close>
+    using pre_Sa
+    unfolding mark_to_delete_clauses_l_pre_def by blast
+
+  have corr_S: \<open>correct_watching S\<close> and
+    blits_S: \<open>blits_in_\<L>\<^sub>i\<^sub>n S\<close> and
+    S_Sa: \<open>(S, Sa) \<in> state_wl_l None\<close>
+    using S_Sa by auto
+  have corr_S: \<open>correct_watching' S\<close>
+    using correct_watching_correct_watching[OF corr_S] .
+  have eq: \<open>set_mset (all_init_lits_of_wl S) = set_mset (all_lits_st S)\<close>
+    using literals_are_\<L>\<^sub>i\<^sub>n'_literals_are_\<L>\<^sub>i\<^sub>n_iff(4)[OF S_Sa Sa_x struct] .
+
+  then have corr_S': \<open>correct_watching S\<close>
+    using corr_S
+    by (cases S; simp only: correct_watching'.simps correct_watching.simps)
+
+  have \<open>literals_are_\<L>\<^sub>i\<^sub>n' S\<close>
+    using blits_S eq
+    unfolding blits_in_\<L>\<^sub>i\<^sub>n_def blits_in_\<L>\<^sub>i\<^sub>n'_def all_lits_def literals_are_\<L>\<^sub>i\<^sub>n'_def
+      all_init_lits_def all_lits_st_init_learned[of S] by auto
+  then show ?thesis
+    using S_Sa corr_S' blits_S
+    unfolding mark_to_delete_clauses_wl_post_def
+    by blast
+qed
+
+lemma cdcl_twl_full_restart_wl_prog_cdcl_full_twl_restart_l_prog:
+  \<open>(cdcl_twl_full_restart_wl_prog, cdcl_twl_full_restart_l_prog)
+    \<in> {(S, T). (S, T) \<in> state_wl_l None \<and> correct_watching S \<and> blits_in_\<L>\<^sub>i\<^sub>n S} \<rightarrow>\<^sub>f
+      \<langle>{(S, T). (S, T) \<in> state_wl_l None \<and> correct_watching S \<and> blits_in_\<L>\<^sub>i\<^sub>n S}\<rangle>nres_rel\<close>
+  unfolding cdcl_twl_full_restart_wl_prog_def cdcl_twl_full_restart_l_prog_def
+    rewatch_clauses_def
+  apply (intro frefI nres_relI)
+  apply (refine_vcg
+     mark_to_delete_clauses_wl_mark_to_delete_clauses_l[THEN fref_to_Down]
+     remove_one_annot_true_clause_imp_wl_remove_one_annot_true_clause_imp[THEN fref_to_Down])
+  subgoal unfolding mark_to_delete_clauses_wl_pre_def
+   by (blast intro: correct_watching_correct_watching mark_to_delete_clauses_l_pre_blits_in_\<L>\<^sub>i\<^sub>n')
+  subgoal unfolding mark_to_delete_clauses_wl_pre_def by (blast intro: correct_watching_correct_watching)
+  subgoal
+    by (rule cdcl_twl_full_restart_wl_prog_final_rel')
+  subgoal by (auto simp: state_wl_l_def mark_to_delete_clauses_wl_post_def)
+  done
+
+definition (in -) restart_abs_wl_pre :: \<open>'v twl_st_wl \<Rightarrow> nat \<Rightarrow> nat \<Rightarrow> bool \<Rightarrow> bool\<close> where
+  \<open>restart_abs_wl_pre S last_GC last_Restart brk \<longleftrightarrow>
+    (\<exists>S'. (S, S') \<in> state_wl_l None \<and> restart_abs_l_pre S' last_GC last_Restart brk
+      \<and> correct_watching S \<and> blits_in_\<L>\<^sub>i\<^sub>n S)\<close>
+
+definition (in -) cdcl_twl_local_restart_wl_spec :: \<open>'v twl_st_wl \<Rightarrow> 'v twl_st_wl nres\<close> where
+  \<open>cdcl_twl_local_restart_wl_spec = (\<lambda>(M, N, D, NE, UE, NS, US, N0, U0, Q, W). do {
+      ASSERT(\<exists>last_GC last_Restart. restart_abs_wl_pre (M, N, D, NE, UE, NS, US, N0, U0, Q, W) last_GC last_Restart False);
+      (M, Q) \<leftarrow> SPEC(\<lambda>(M', Q'). (\<exists>K M2. (Decided K # M', M2) \<in> set (get_all_ann_decomposition M) \<and>
+            Q' = {#}) \<or> (M' = M \<and> Q' = Q));
+      RETURN (M, N, D, NE, UE, NS, US, N0, U0, Q, W)
+   })\<close>
+
+lemma cdcl_twl_local_restart_wl_spec_cdcl_twl_local_restart_l_spec:
+  \<open>(cdcl_twl_local_restart_wl_spec, cdcl_twl_local_restart_l_spec)
+    \<in> {(S, T). (S, T) \<in> state_wl_l None \<and> correct_watching S \<and> blits_in_\<L>\<^sub>i\<^sub>n S} \<rightarrow>\<^sub>f
+      \<langle>{(S, T). (S, T) \<in> state_wl_l None \<and> correct_watching S \<and> blits_in_\<L>\<^sub>i\<^sub>n S}\<rangle>nres_rel\<close>
+proof -
+  have [simp]:
+    \<open>all_lits N (NE + UE + (NS + US) + (N0 + U0)) = all_lits N (NE + UE + NS + US + N0 + U0)\<close>
+    \<open>all_lits N ((NE + UE) + (NS + US) + (N0 + U0)) = all_lits N (NE + UE + NS + US + N0 + U0)\<close>
+    for NE UE NS US N
+    by (auto simp: ac_simps)
+  have [refine0]:
+    \<open>\<And>x y x1 x2 x1a x2a x1b x2b x1c x2c x1d x2d x1e x2e x1f x2f x1g x2g x1h x2h x1i x2i x1j x2j x1k
+    x2k y1f y2g y2g y1h y1i x2m x1l x1n x2o y2i x1o x1p x2p x1q x2q y2i y1i y2j y1j y2k x2r x1q
+    y1k y2l x1k.
+        (x, y) \<in> {(S, T). (S, T) \<in> state_wl_l None \<and> correct_watching S \<and> blits_in_\<L>\<^sub>i\<^sub>n S} \<Longrightarrow>
+        y2j = (y1j, y2k) \<Longrightarrow>
+        y2i = (y1i, y2j) \<Longrightarrow>
+        y2g = (y1h, y2i) \<Longrightarrow>
+        x2e = (y1f, y2g) \<Longrightarrow>
+        x2d = (x1e, x2e) \<Longrightarrow>
+        x2c = (x1d, x2d) \<Longrightarrow>
+        x2b = (x1c, x2c) \<Longrightarrow>
+        x2a = (x1b, x2b) \<Longrightarrow>
+        x2 = (x1a, x2a) \<Longrightarrow>
+        y = (x1, x2) \<Longrightarrow>
+        x2p = (x1p, x2q) \<Longrightarrow>
+        x2o = (x1o, x2p) \<Longrightarrow>
+        x2m = (x1n, x2o) \<Longrightarrow>
+        x2k = (x1l, x2m) \<Longrightarrow>
+        x2j = (x1k, x2k) \<Longrightarrow>
+        x2i = (x1j, x2j) \<Longrightarrow>
+        x2h = (x1i, x2i) \<Longrightarrow>
+        x2g = (x1h, x2h) \<Longrightarrow>
+        x2f = (x1g, x2g) \<Longrightarrow>
+        x = (x1f, x2f) \<Longrightarrow>
+        SPEC (\<lambda>(M', Q'). (\<exists>K M2. (Decided K # M', M2) \<in> set (get_all_ann_decomposition x1f) \<and>
+           Q' = {#}) \<or> M' = x1f \<and> Q' = x1p)
+        \<le> \<Down>Id (SPEC (\<lambda>(M', Q') .(\<exists>K M2. (Decided K # M', M2) \<in> set (get_all_ann_decomposition x1) \<and>
+    Q' = {#}) \<or> M' = x1 \<and> Q' = y2k))\<close>
+    by (auto 5 3 simp: state_wl_l_def)
+  show ?thesis
+    unfolding cdcl_twl_local_restart_wl_spec_def cdcl_twl_local_restart_l_spec_def
+      rewatch_clauses_def
+    apply (intro frefI nres_relI)
+    apply (refine_vcg)
+    subgoal unfolding restart_abs_wl_pre_def by fast
+    apply assumption+
+    subgoal
+      by (fastforce simp: state_wl_l_def correct_watching.simps clause_to_update_def
+          blits_in_\<L>\<^sub>i\<^sub>n_def
+        simp flip: all_lits_alt_def2)
+    done
+qed
+
+definition cdcl_twl_restart_wl_prog where
+\<open>cdcl_twl_restart_wl_prog S = do {
+   cdcl_twl_local_restart_wl_spec S
+  }\<close>
+
+lemma cdcl_twl_restart_wl_prog_cdcl_twl_restart_l_prog:
+  \<open>(cdcl_twl_restart_wl_prog, cdcl_twl_restart_l_prog)
+    \<in> {(S, T). (S, T) \<in> state_wl_l None \<and> correct_watching S \<and> blits_in_\<L>\<^sub>i\<^sub>n S} \<rightarrow>\<^sub>f
+      \<langle>{(S, T). (S, T) \<in> state_wl_l None \<and> correct_watching S \<and> blits_in_\<L>\<^sub>i\<^sub>n S}\<rangle>nres_rel\<close>
+  unfolding cdcl_twl_restart_wl_prog_def cdcl_twl_restart_l_prog_def
+    rewatch_clauses_def
+  apply (intro frefI nres_relI)
+  apply (refine_vcg cdcl_twl_local_restart_wl_spec_cdcl_twl_local_restart_l_spec[THEN fref_to_Down])
+  done
+
+
+datatype restart_type =
+  NO_RESTART |
+  GC |
+  RESTART
+
+context twl_restart_ops
+begin
+
+definition (in twl_restart_ops) restart_required_wl  :: \<open>'v twl_st_wl \<Rightarrow> nat \<Rightarrow> nat \<Rightarrow> nat \<Rightarrow> restart_type nres\<close> where
+\<open>restart_required_wl S last_GC last_Restart n =  do {
+  ASSERT(size (get_all_learned_clss_wl S) \<ge> last_GC);
+  ASSERT(size (get_all_learned_clss_wl S) \<ge> last_Restart);
+  SPEC (\<lambda>b.
+  (b = GC \<longrightarrow> f n < size (get_all_learned_clss_wl S) - last_GC) \<and>
+  (b = RESTART \<longrightarrow> last_Restart < size (get_all_learned_clss_wl S)))}\<close>
+
+definition (in twl_restart_ops) cdcl_twl_stgy_restart_abs_wl_inv
+   :: \<open>'v twl_st_wl \<Rightarrow> bool \<times> 'v twl_st_wl \<times> nat \<times> nat \<times> nat \<Rightarrow> bool\<close> where
+  \<open>cdcl_twl_stgy_restart_abs_wl_inv S\<^sub>0 = (\<lambda>(brk, T, last_GC, last_Restart, n).
+    (\<exists>S\<^sub>0' T'.
+       (S\<^sub>0, S\<^sub>0') \<in> state_wl_l None \<and>
+       (T, T') \<in> state_wl_l None \<and>
+       cdcl_twl_stgy_restart_abs_l_inv S\<^sub>0' (brk, T', last_GC, last_Restart, n) \<and>
+       correct_watching T))\<close>
+end
+
+
+context twl_restart_ops
+begin
+
+definition cdcl_GC_clauses_pre_wl :: \<open>'v twl_st_wl \<Rightarrow> bool\<close> where
+\<open>cdcl_GC_clauses_pre_wl S \<longleftrightarrow> (
+  \<exists>T. (S, T) \<in> state_wl_l None \<and>
+    correct_watching'' S \<and>
+    literals_are_\<L>\<^sub>i\<^sub>n' S \<and>
+    cdcl_GC_clauses_pre T
+  )\<close>
+
+definition cdcl_GC_clauses_wl :: \<open>'v twl_st_wl \<Rightarrow> 'v twl_st_wl nres\<close> where
+\<open>cdcl_GC_clauses_wl = (\<lambda>(M, N, D, NE, UE, NS, US, N0, U0, WS, Q). do {
+  ASSERT(cdcl_GC_clauses_pre_wl (M, N, D, NE, UE, NS, US, N0, U0, WS, Q));
+  let b = True;
+  if b then do {
+    (N', _) \<leftarrow> SPEC (\<lambda>(N'', m). GC_remap\<^sup>*\<^sup>* (N, Map.empty, fmempty) (fmempty, m, N'') \<and>
+      0 \<notin># dom_m N'');
+    Q \<leftarrow> SPEC(\<lambda>Q. correct_watching' (M, N', D, NE, UE, NS, US, N0, U0, WS, Q)\<and> literals_are_\<L>\<^sub>i\<^sub>n' (M, N', D, NE, UE, NS, US, N0, U0, WS, Q));
+    RETURN (M, N', D, NE, UE, NS, {#}, N0, U0, WS, Q)
+  }
+  else RETURN (M, N, D, NE, UE, NS, {#}, N0, U0, WS, Q)})\<close>
+
+lemma literals_are_\<L>\<^sub>i\<^sub>n'_empty:
+  \<open>NO_MATCH {#} x2m \<Longrightarrow> literals_are_\<L>\<^sub>i\<^sub>n' (x1h, x1p, x1j, x1k, b, x', x2l, N0, U0, x2m, Q) \<longleftrightarrow>
+     literals_are_\<L>\<^sub>i\<^sub>n' (x1h, x1p, x1j, x1k, b, x', x2l, N0, U0, {#}, Q)\<close>
+   \<open>NO_MATCH {#} x2l \<Longrightarrow> correct_watching' (x1h, x1i, x1j, x1k, b, x', x2l, N0, U0, x2m, Q) \<longleftrightarrow>
+    correct_watching' (x1h, x1i, x1j, x1k, b, x', {#}, N0, U0, x2m, Q)\<close>
+   \<open>NO_MATCH {#} x2m \<Longrightarrow> correct_watching' (x1h, x1i, x1j, x1k, b, x', x2l, N0, U0, x2m, Q) \<longleftrightarrow>
+    correct_watching' (x1h, x1i, x1j, x1k, b, x', x2l, N0, U0, {#}, Q)\<close>
+  \<open>literals_are_\<L>\<^sub>i\<^sub>n' (x1h, x1p, x1j, x1k, b, x', x2l, N0, U0, x2m, Q) \<Longrightarrow>
+     literals_are_\<L>\<^sub>i\<^sub>n' (x1h, x1p, x1j, x1k, b, x', {#}, N0, U0, x2m, Q)\<close>
+   by (auto 5 3 simp: literals_are_\<L>\<^sub>i\<^sub>n'_def blits_in_\<L>\<^sub>i\<^sub>n'_def all_lits_of_mm_union
+     correct_watching'.simps correct_watching''.simps clause_to_update_def all_init_lits_of_wl_def
+     all_learned_lits_of_wl_def)
+
+lemma literals_are_\<L>\<^sub>i\<^sub>n'_decompD:
+  \<open>(K # x1h', M2) \<in> set (get_all_ann_decomposition x1h) \<Longrightarrow>
+  literals_are_\<L>\<^sub>i\<^sub>n' (x1h, x1p, x1j', x1k, b, x', x2l, N0, U0, x2m, Q) \<Longrightarrow>
+     literals_are_\<L>\<^sub>i\<^sub>n' (x1h', x1p, x1j, x1k, b, x', x2l, N0, U0, x2m, Q)\<close>
+  by (auto 5 3 simp: literals_are_\<L>\<^sub>i\<^sub>n'_def blits_in_\<L>\<^sub>i\<^sub>n'_def all_lits_of_mm_union
+     correct_watching'.simps correct_watching''.simps clause_to_update_def all_init_lits_of_wl_def
+     all_learned_lits_of_wl_def
+     dest!: get_all_ann_decomposition_exists_prepend)
+
+lemma cdcl_GC_clauses_wl_cdcl_GC_clauses:
+  \<open>(cdcl_GC_clauses_wl, cdcl_GC_clauses) \<in> {(S::'v twl_st_wl, S').
+       (S, S') \<in> state_wl_l None \<and> correct_watching'' S \<and> literals_are_\<L>\<^sub>i\<^sub>n' S} \<rightarrow>\<^sub>f \<langle>{(S::'v twl_st_wl, S').
+       (S, S') \<in> state_wl_l None \<and> correct_watching' S \<and> literals_are_\<L>\<^sub>i\<^sub>n' S}\<rangle>nres_rel\<close>
+  unfolding cdcl_GC_clauses_wl_def cdcl_GC_clauses_def
+  apply (intro frefI nres_relI)
+  apply refine_vcg
+  subgoal unfolding cdcl_GC_clauses_pre_wl_def by blast
+  subgoal by (auto simp: state_wl_l_def)
+  subgoal by (auto simp: state_wl_l_def)
+  subgoal by auto
+  subgoal for x y x1 x2 x1a x2a x1b x2b x1c x2c x1d x2d x1e x2e x1f x2f x1g x2g x1h
+       x2h x1i x2i x1j x2j x1k x2k b xa x' x1l x2l x1m x2m Q
+    by (auto simp: state_wl_l_def blits_in_\<L>\<^sub>i\<^sub>n'_def literals_are_\<L>\<^sub>i\<^sub>n'_empty
+      dest: multi_member_split)
+  subgoal by auto
+  done
+
+definition cdcl_twl_full_restart_wl_GC_prog_post :: \<open>'v twl_st_wl \<Rightarrow> 'v twl_st_wl \<Rightarrow> bool\<close> where
+\<open>cdcl_twl_full_restart_wl_GC_prog_post S T \<longleftrightarrow>
+  (\<exists>S' T'. (S, S') \<in> state_wl_l None \<and> (T, T') \<in> state_wl_l None \<and>
+    cdcl_twl_full_restart_l_GC_prog_pre S' \<and>
+    cdcl_twl_restart_l S' T' \<and> correct_watching' T \<and>
+    set_mset (all_init_lits_of_wl T) =
+    set_mset (all_lits_st T))\<close>
+
+definition (in -) restart_abs_wl_pre2 :: \<open>'v twl_st_wl \<Rightarrow> bool \<Rightarrow> bool\<close> where
+  \<open>restart_abs_wl_pre2 S brk \<longleftrightarrow>
+    (\<exists>S' last_GC last_Restart. (S, S') \<in> state_wl_l None \<and> restart_abs_l_pre S' last_GC last_Restart brk
+      \<and> correct_watching'' S \<and> literals_are_\<L>\<^sub>i\<^sub>n' S)\<close>
+
+definition (in -) cdcl_twl_local_restart_wl_spec0 :: \<open>'v twl_st_wl \<Rightarrow> 'v twl_st_wl nres\<close> where
+  \<open>cdcl_twl_local_restart_wl_spec0 = (\<lambda>(M, N, D, NE, UE, NS, US, N0, U0, Q, W). do {
+      ASSERT(restart_abs_wl_pre2 (M, N, D, NE, UE, NS, US, N0, U0, Q, W) False);
+      (M, Q) \<leftarrow> SPEC(\<lambda>(M', Q'). (\<exists>K M2. (Decided K # M', M2) \<in> set (get_all_ann_decomposition M) \<and>
+            Q' = {#} \<and> count_decided M' = 0) \<or> (M' = M \<and> Q' = Q \<and> count_decided M' = 0));
+      RETURN (M, N, D, NE, UE, NS, {#}, N0, U0, Q, W)
+   })\<close>
+
+
+definition mark_to_delete_clauses_wl2_inv
+  :: \<open>'v twl_st_wl \<Rightarrow> nat list \<Rightarrow> nat \<times> 'v twl_st_wl\<times> nat list  \<Rightarrow> bool\<close>
+where
+  \<open>mark_to_delete_clauses_wl2_inv = (\<lambda>S xs0 (i, T, xs).
+     \<exists>S' T'. (S, S') \<in> state_wl_l None \<and> (T, T') \<in> state_wl_l None \<and>
+      mark_to_delete_clauses_l_inv S' xs0 (i, T', xs) \<and>
+      correct_watching'' S \<and> literals_are_\<L>\<^sub>i\<^sub>n' S \<and> literals_are_\<L>\<^sub>i\<^sub>n' T)\<close>
+
+
+(*TODO What is exactly the difference with mark_to_delete_clauses_wl?*)
+definition mark_to_delete_clauses_wl2 :: \<open>'v twl_st_wl \<Rightarrow> 'v twl_st_wl nres\<close> where
+\<open>mark_to_delete_clauses_wl2  = (\<lambda>S. do {
+    ASSERT(mark_to_delete_clauses_wl_pre S);
+    xs \<leftarrow> collect_valid_indices_wl S;
+    l \<leftarrow> SPEC(\<lambda>_:: nat. True);
+    (_, S, _) \<leftarrow> WHILE\<^sub>T\<^bsup>mark_to_delete_clauses_wl2_inv S xs\<^esup>
+      (\<lambda>(i, S, xs). i < length xs)
+      (\<lambda>(i, T, xs). do {
+        if(xs!i \<notin># dom_m (get_clauses_wl T)) then RETURN (i, T, delete_index_and_swap xs i)
+        else do {
+          ASSERT(0 < length (get_clauses_wl T\<propto>(xs!i)));
+	  ASSERT (get_clauses_wl T \<propto> (xs ! i) ! 0 \<in># \<L>\<^sub>a\<^sub>l\<^sub>l (all_init_atms_st T));
+          can_del \<leftarrow> SPEC(\<lambda>b. b \<longrightarrow>
+             (Propagated (get_clauses_wl T\<propto>(xs!i)!0) (xs!i) \<notin> set (get_trail_wl T)) \<and>
+              \<not>irred (get_clauses_wl T) (xs!i) \<and> length (get_clauses_wl T \<propto> (xs!i)) \<noteq> 2);
+          ASSERT(i < length xs);
+          if can_del
+          then
+            RETURN (i, mark_garbage_wl (xs!i) T, delete_index_and_swap xs i)
+          else
+            RETURN (i+1, T, xs)
+       }
+      })
+      (l, S, xs);
+    remove_all_learned_subsumed_clauses_wl S
+  })\<close>
+
+lemma mark_to_delete_clauses_wl2_invD1:
+  assumes \<open>mark_to_delete_clauses_wl2_inv S xs (i, T, ys)\<close> and
+    \<open>C \<in># dom_m (get_clauses_wl T)\<close> and
+    \<open>0 < length (get_clauses_wl T \<propto> C)\<close>
+  shows
+    \<open>get_clauses_wl T \<propto> C ! 0 \<in># \<L>\<^sub>a\<^sub>l\<^sub>l (all_init_atms_st T)\<close>
+proof -
+  have \<open>get_clauses_wl T \<propto> C ! 0 \<in># all_lits_st T\<close>
+    using assms(2,3) by auto
+  moreover have \<open>literals_are_\<L>\<^sub>i\<^sub>n' T\<close>
+    using assms unfolding mark_to_delete_clauses_wl2_inv_def by blast
+  ultimately show \<open>?thesis\<close>
+    unfolding all_lits_st_init_learned \<L>\<^sub>a\<^sub>l\<^sub>l_all_init_atms literals_are_\<L>\<^sub>i\<^sub>n'_def
+    by auto
+qed
+
+lemma mark_to_delete_clauses_wl_mark_to_delete_clauses_l2:
+  \<open>(mark_to_delete_clauses_wl2, mark_to_delete_clauses_l)
+    \<in> {(S, T). (S, T) \<in> state_wl_l None \<and> correct_watching'' S \<and> literals_are_\<L>\<^sub>i\<^sub>n' S} \<rightarrow>\<^sub>f
+      \<langle>{(S, T). (S, T) \<in> state_wl_l None \<and> correct_watching'' S \<and> literals_are_\<L>\<^sub>i\<^sub>n' S}\<rangle>nres_rel\<close>
+proof -
+  have [refine0]: \<open>collect_valid_indices_wl S  \<le> \<Down> Id (collect_valid_indices S')\<close>
+    if \<open>(S, S') \<in> {(S, T).  (S, T) \<in> state_wl_l None \<and> correct_watching'' S \<and>
+           mark_to_delete_clauses_wl_pre S}\<close>
+    for S S'
+    using that by (auto simp: collect_valid_indices_wl_def collect_valid_indices_def)
+  have if_inv: \<open>(if A then RETURN P else RETURN Q) = RETURN (if A then P else Q)\<close> for A P Q
+    by auto
+  have Ball_range[simp]: \<open>(\<forall>x\<in>range f \<union> range g. P x)\<longleftrightarrow>(\<forall>x. P (f x) \<and> P (g x))\<close> for P f g
+    by auto
+  show ?thesis
+    unfolding mark_to_delete_clauses_wl2_def mark_to_delete_clauses_l_def
+      uncurry_def
+    apply (intro frefI nres_relI)
+    apply (refine_vcg
+      WHILEIT_refine[where
+         R = \<open>{((i, S, xs), (j, T, ys)). i = j \<and> (S, T) \<in> state_wl_l None \<and> correct_watching'' S \<and>
+             xs = ys \<and> literals_are_\<L>\<^sub>i\<^sub>n' S}\<close>]
+      remove_one_annot_true_clause_one_imp_wl_remove_one_annot_true_clause_one_imp[THEN fref_to_Down_curry]
+      remove_all_learned_subsumed_clauses_wl_remove_all_learned_subsumed_clauses[THEN fref_to_Down])
+    subgoal unfolding mark_to_delete_clauses_wl_pre_def by blast
+    subgoal by auto
+    subgoal by (auto simp: state_wl_l_def)
+    subgoal unfolding mark_to_delete_clauses_wl2_inv_def by fast
+    subgoal by auto
+    subgoal by (force simp: state_wl_l_def)
+    subgoal by auto
+    subgoal by (force simp: state_wl_l_def)
+    subgoal for x y xs xsa l to_keep xa x' x1 x2 x1a x2a x1b x2b x1c x2c
+      by (auto simp: mark_to_delete_clauses_wl2_invD1)
+    subgoal by (auto simp: state_wl_l_def can_delete_def)
+    subgoal by auto
+    subgoal by (force simp: state_wl_l_def)
+    subgoal
+      by (auto simp: state_wl_l_def correct_watching_fmdrop mark_garbage_wl_def
+          mark_garbage_l_def correct_watching''_fmdrop
+        split: prod.splits)
+    subgoal by (auto simp: state_wl_l_def)
+    subgoal by (auto simp: ac_simps)
+    done
+qed
+
+definition cdcl_twl_full_restart_wl_GC_prog_pre
+  :: \<open>'v twl_st_wl \<Rightarrow> bool\<close>
+where
+  \<open>cdcl_twl_full_restart_wl_GC_prog_pre S \<longleftrightarrow>
+   (\<exists>T. (S, T) \<in> state_wl_l None \<and> correct_watching' S \<and> literals_are_\<L>\<^sub>i\<^sub>n' S \<and> cdcl_twl_full_restart_l_GC_prog_pre T)\<close>
+
+definition cdcl_twl_full_restart_wl_GC_prog where
+\<open>cdcl_twl_full_restart_wl_GC_prog S = do {
+    ASSERT(cdcl_twl_full_restart_wl_GC_prog_pre S);
+    S' \<leftarrow> cdcl_twl_local_restart_wl_spec0 S;
+    T \<leftarrow> remove_one_annot_true_clause_imp_wl S';
+    ASSERT(mark_to_delete_clauses_wl_pre T);
+    U \<leftarrow> mark_to_delete_clauses_wl2 T;
+    V \<leftarrow> cdcl_GC_clauses_wl U;
+    ASSERT(cdcl_twl_full_restart_wl_GC_prog_post S V);
+    RETURN V
+  }\<close>
+
+lemma blits_in_\<L>\<^sub>i\<^sub>n'_restart_wl_spec0:
+  \<open>NO_MATCH {#} f' \<Longrightarrow>
+  literals_are_\<L>\<^sub>i\<^sub>n' (a, b, c, d, e, NS, US, N0, U0, f', g) \<longleftrightarrow>
+      literals_are_\<L>\<^sub>i\<^sub>n' (ah, b, c, d, e, NS, US, N0, U0, {#}, g)\<close>
+  by (auto simp: blits_in_\<L>\<^sub>i\<^sub>n'_def literals_are_\<L>\<^sub>i\<^sub>n'_def
+         all_init_lits_def all_init_lits_of_wl_def all_learned_lits_of_wl_def)
+
+lemma all_init_lits_of_wl_keepUSD:
+  \<open>L \<in># all_init_lits_of_wl ([], x1k, x1l, x1m, x1n, x1o, {#}, x1q, x1r, {#}, x2s) \<Longrightarrow>
+  L \<in># all_init_lits_of_wl ([], x1k, x1l, x1m, x1n, x1o, {#}, x1q, x1r, Q, x2s)\<close>
+  by (auto simp: all_init_lits_of_wl_def all_lits_of_mm_def)
+
+lemma all_init_learned_lits_simps_Q:
+  \<open>NO_MATCH {#} Q \<Longrightarrow> all_init_lits_of_wl (M, N, D, NE, UE, NS, US, N0, U0, Q, W) =
+    all_init_lits_of_wl (M, N, D, NE, UE, NS, US, N0, U0, {#}, W)\<close>
+  \<open>NO_MATCH {#} Q \<Longrightarrow> all_learned_lits_of_wl (M, N, D, NE, UE, NS, US, N0, U0, Q, W) =
+    all_learned_lits_of_wl (M, N, D, NE, UE, NS, US, N0, U0, {#}, W)\<close>
+  by (auto simp: all_init_lits_of_wl_def all_learned_lits_of_wl_def all_lits_of_mm_def)
+  
+lemma cdcl_twl_local_restart_wl_spec0_cdcl_twl_local_restart_l_spec0:
+  \<open>(x, y) \<in> {(S, S'). (S, S') \<in> state_wl_l None \<and> correct_watching'' S \<and> literals_are_\<L>\<^sub>i\<^sub>n' S} \<Longrightarrow>
+          cdcl_twl_local_restart_wl_spec0 x
+          \<le> \<Down> {(S, S'). (S, S') \<in> state_wl_l None \<and> correct_watching'' S \<and> literals_are_\<L>\<^sub>i\<^sub>n' S}
+	    (cdcl_twl_local_restart_l_spec0 y)\<close>
+  unfolding cdcl_twl_local_restart_wl_spec0_def cdcl_twl_local_restart_l_spec0_def curry_def
+  apply refine_vcg
+  subgoal unfolding restart_abs_wl_pre2_def by (rule exI[of _ y]) fast
+  subgoal
+    by (auto simp add: literals_are_\<L>\<^sub>i\<^sub>n'_empty
+        state_wl_l_def image_iff correct_watching''.simps clause_to_update_def
+      conc_fun_RES RES_RETURN_RES2 blits_in_\<L>\<^sub>i\<^sub>n'_restart_wl_spec0
+      intro: literals_are_\<L>\<^sub>i\<^sub>n'_decompD literals_are_\<L>\<^sub>i\<^sub>n'_empty(4))
+  subgoal
+    by (auto simp add: literals_are_\<L>\<^sub>i\<^sub>n'_empty
+        state_wl_l_def image_iff correct_watching''.simps clause_to_update_def
+      conc_fun_RES RES_RETURN_RES2 blits_in_\<L>\<^sub>i\<^sub>n'_restart_wl_spec0
+      literals_are_\<L>\<^sub>i\<^sub>n'_def all_init_learned_lits_simps_Q blits_in_\<L>\<^sub>i\<^sub>n'_def
+      dest: all_init_lits_of_wl_keepUSD)
+  done
+
+lemma (in -)[twl_st,simp]: \<open>learned_clss (state\<^sub>W_of S) = get_all_learned_clss S\<close>
+  by (cases S) auto
+
+lemma (in -)[twl_st,simp]: \<open>init_clss (state\<^sub>W_of S) = get_all_init_clss S\<close>
+  by (cases S) auto
+
+lemma cdcl_twl_full_restart_wl_GC_prog_post_correct_watching:
+  assumes
+    pre: \<open>cdcl_twl_full_restart_l_GC_prog_pre y\<close> and
+    y_Va: \<open>cdcl_twl_restart_l y Va\<close>
+    \<open>(V, Va) \<in> {(S, S'). (S, S') \<in> state_wl_l None \<and> correct_watching' S \<and> literals_are_\<L>\<^sub>i\<^sub>n' S}\<close>
+  shows \<open>(V, Va) \<in> {(S, S'). (S, S') \<in> state_wl_l None \<and> correct_watching S \<and> blits_in_\<L>\<^sub>i\<^sub>n S}\<close> and
+    \<open>set_mset (all_init_lits_of_wl V) = set_mset (all_lits_st V)\<close>
+proof -
+  obtain x where
+    y_x: \<open>(y, x) \<in> twl_st_l None\<close> and
+    struct_invs: \<open>twl_struct_invs x\<close> and
+    list_invs: \<open>twl_list_invs y\<close>
+    using pre unfolding cdcl_twl_full_restart_l_GC_prog_pre_def by blast
+  obtain V' where \<open>cdcl_twl_restart x V'\<close> and Va_V': \<open>(Va, V') \<in> twl_st_l None\<close>
+    using cdcl_twl_restart_l_cdcl_twl_restart[OF y_x list_invs struct_invs] y_Va
+    unfolding conc_fun_RES by auto
+  then have \<open>twl_struct_invs V'\<close>
+    using struct_invs by (blast dest: cdcl_twl_restart_twl_struct_invs)
+  then show eq: \<open>set_mset (all_init_lits_of_wl V) = set_mset (all_lits_st V)\<close>
+    using assms(3) Va_V'  \<open>twl_struct_invs V'\<close> literals_are_\<L>\<^sub>i\<^sub>n'_literals_are_\<L>\<^sub>i\<^sub>n_iff(4) by blast
+  then have \<open>correct_watching' V \<Longrightarrow>  correct_watching V\<close>
+    by (cases V) (auto simp: correct_watching.simps correct_watching'.simps)
+  moreover
+    have \<open>literals_are_\<L>\<^sub>i\<^sub>n' V \<Longrightarrow> blits_in_\<L>\<^sub>i\<^sub>n V\<close>
+    using eq by (cases V)
+      (clarsimp simp: blits_in_\<L>\<^sub>i\<^sub>n_def blits_in_\<L>\<^sub>i\<^sub>n'_def all_lits_def literals_are_\<L>\<^sub>i\<^sub>n'_def
+         all_init_lits_def ac_simps)
+  ultimately show \<open>(V, Va) \<in> {(S, S'). (S, S') \<in> state_wl_l None \<and> correct_watching S \<and> blits_in_\<L>\<^sub>i\<^sub>n S}\<close>
+    using assms by (auto simp: cdcl_twl_full_restart_wl_GC_prog_post_def)
+qed
+
+lemma cdcl_twl_full_restart_wl_GC_prog:
+  \<open>(cdcl_twl_full_restart_wl_GC_prog, cdcl_twl_full_restart_l_GC_prog) \<in> {(S::'v twl_st_wl, S').
+       (S, S') \<in> state_wl_l None \<and> correct_watching' S \<and> literals_are_\<L>\<^sub>i\<^sub>n' S} \<rightarrow>\<^sub>f \<langle>{(S::'v twl_st_wl, S').
+       (S, S') \<in> state_wl_l None \<and> correct_watching S \<and> blits_in_\<L>\<^sub>i\<^sub>n S}\<rangle>nres_rel\<close>
+  unfolding cdcl_twl_full_restart_wl_GC_prog_def cdcl_twl_full_restart_l_GC_prog_def
+  apply (intro frefI nres_relI)
+  apply (refine_vcg
+    remove_one_annot_true_clause_imp_wl_remove_one_annot_true_clause_imp[THEN fref_to_Down]
+    mark_to_delete_clauses_wl_mark_to_delete_clauses_l2[THEN fref_to_Down]
+    cdcl_GC_clauses_wl_cdcl_GC_clauses[THEN fref_to_Down]
+    cdcl_twl_local_restart_wl_spec0_cdcl_twl_local_restart_l_spec0)
+  subgoal unfolding cdcl_twl_full_restart_wl_GC_prog_pre_def by blast
+  subgoal by (auto dest: correct_watching'_correct_watching'')
+  subgoal unfolding mark_to_delete_clauses_wl_pre_def by fast
+  subgoal for x y S S' T Ta U Ua V Va
+    using cdcl_twl_full_restart_wl_GC_prog_post_correct_watching[of y Va V]
+    unfolding cdcl_twl_full_restart_wl_GC_prog_post_def
+    by fast
+  subgoal for x y S' S'a T Ta U Ua V Va
+    by (rule cdcl_twl_full_restart_wl_GC_prog_post_correct_watching)
+  done
+
+definition (in twl_restart_ops) restart_prog_wl
+  :: "'v twl_st_wl \<Rightarrow> nat \<Rightarrow> nat \<Rightarrow> nat \<Rightarrow> bool \<Rightarrow> ('v twl_st_wl \<times> nat \<times> nat \<times> nat) nres"
+where
+  \<open>restart_prog_wl S last_GC last_Restart n brk = do {
+     ASSERT(restart_abs_wl_pre S last_GC last_Restart brk);
+     b \<leftarrow> restart_required_wl S last_GC last_Restart n;
+      if b = RESTART \<and> \<not>brk then do {
+       T \<leftarrow> cdcl_twl_restart_wl_prog S;
+       RETURN (T, last_GC, size (get_all_learned_clss_wl T), n)
+     }
+     else if b = GC \<and> \<not>brk then do {
+       b \<leftarrow> SPEC(\<lambda>_. True);
+       T \<leftarrow> (if b then cdcl_twl_full_restart_wl_prog S else cdcl_twl_full_restart_wl_GC_prog S);
+       RETURN (T, size (get_all_learned_clss_wl T), size (get_all_learned_clss_wl T), n + 1)
+     }
+     else
+       RETURN (S, last_GC, last_Restart, n)
+   }\<close>
+
+lemma restart_prog_wl_alt_def:
+ \<open>restart_prog_wl S last_GC last_Restart n brk = do {
+     ASSERT(restart_abs_wl_pre S last_GC last_Restart brk);
+     b \<leftarrow> restart_required_wl S last_GC last_Restart n;
+     let _ = (b = RESTART);
+      if b = RESTART \<and> \<not>brk then do {
+       T \<leftarrow> cdcl_twl_restart_wl_prog S;
+       RETURN (T, last_GC, size (get_all_learned_clss_wl T), n)
+     }
+     else if b = GC \<and> \<not>brk then do {
+       b \<leftarrow> SPEC(\<lambda>_. True);
+       T \<leftarrow> (if b then cdcl_twl_full_restart_wl_prog S else cdcl_twl_full_restart_wl_GC_prog S);
+       RETURN (T, size (get_all_learned_clss_wl T), size (get_all_learned_clss_wl T), n + 1)
+     }
+     else
+       RETURN (S, last_GC, last_Restart, n)
+   }\<close>
+  unfolding restart_prog_wl_def
+  by auto
+
+lemma restart_abs_wl_pre_blits_in_\<L>\<^sub>i\<^sub>n:
+  assumes pre: \<open>restart_abs_wl_pre x1c last_GC last_Restart b\<close> and
+    \<open>blits_in_\<L>\<^sub>i\<^sub>n x1c\<close>
+  shows \<open>literals_are_\<L>\<^sub>i\<^sub>n' x1c\<close>
+proof -
+
+  obtain y x where
+    y_x: \<open>(y, x) \<in> twl_st_l None\<close> and
+    x1c_y: \<open>(x1c, y) \<in> state_wl_l None\<close> and
+    struct_invs: \<open>twl_struct_invs x\<close> and
+    list_invs: \<open>twl_list_invs y\<close>
+    using pre unfolding restart_abs_wl_pre_def restart_abs_l_pre_def
+      restart_prog_pre_def apply - apply normalize_goal+
+    by blast
+  then have eq:
+    \<open>set_mset (all_init_lits_of_wl x1c) = set_mset (all_lits_st x1c)\<close>
+    using y_x x1c_y literals_are_\<L>\<^sub>i\<^sub>n'_literals_are_\<L>\<^sub>i\<^sub>n_iff(4) by blast
+  moreover have eq: \<open>set_mset (all_learned_lits_of_wl x1c) \<subseteq> set_mset (all_lits_st x1c)\<close>
+    using y_x x1c_y
+    unfolding all_lits_st_init_learned by auto
+  ultimately show \<open>literals_are_\<L>\<^sub>i\<^sub>n' x1c\<close>
+    using eq assms by (cases x1c)
+      (clarsimp simp: blits_in_\<L>\<^sub>i\<^sub>n_def blits_in_\<L>\<^sub>i\<^sub>n'_def all_lits_def literals_are_\<L>\<^sub>i\<^sub>n'_def
+         all_init_lits_def ac_simps)
+qed
+
+lemma cdcl_twl_full_restart_wl_prog_cdcl_twl_restart_l_prog:
+  \<open>(uncurry4 restart_prog_wl, uncurry4 restart_prog_l)
+    \<in> {(S, T).  (S, T) \<in> state_wl_l None \<and> correct_watching S \<and> blits_in_\<L>\<^sub>i\<^sub>n S} \<times>\<^sub>f nat_rel\<times>\<^sub>f nat_rel\<times>\<^sub>f nat_rel \<times>\<^sub>f bool_rel \<rightarrow>\<^sub>f
+      \<langle>{(S, T).  (S, T) \<in> state_wl_l None \<and> correct_watching S \<and> blits_in_\<L>\<^sub>i\<^sub>n S} \<times>\<^sub>r nat_rel\<times>\<^sub>r nat_rel\<times>\<^sub>r nat_rel\<rangle>nres_rel\<close>
+    (is \<open>_ \<in> ?R \<times>\<^sub>f _ \<times>\<^sub>f _ \<times>\<^sub>f _ \<times>\<^sub>f _  \<rightarrow>\<^sub>f \<langle>?R'\<rangle>nres_rel\<close>)
+proof -
+  have [simp]: \<open>size (learned_clss_l (get_clauses_wl a)) = size ((get_learned_clss_wl a))\<close> for a
+    by (cases a, auto simp: get_learned_clss_wl_def)
+  have [refine0]:
+    \<open>restart_required_wl a b c d \<le> \<Down> {(b, b'). (b' = (b = GC)) \<and>
+    (b = RESTART \<longrightarrow> size (get_all_learned_clss_wl a) > c)} (GC_required_l a' b' d')\<close>
+    (is \<open>_ \<le> \<Down> ?GC _\<close>)
+    if \<open>(a, a') \<in> ?R\<close> and \<open>(b, b') \<in> nat_rel\<close> \<open>(d, d') \<in> nat_rel\<close>
+      \<open>restart_abs_wl_pre a b c brk\<close>
+    for a a' b b' c c' d d' e e' brk
+    using that unfolding restart_abs_wl_pre_def GC_required_l_def restart_abs_l_pre_def
+      restart_required_wl_def restart_prog_pre_def apply -
+    apply (refine_rcg)
+    subgoal by auto
+    subgoal by normalize_goal+ simp
+    by (rule RES_refine, rule_tac x= \<open>s = GC\<close> in bexI)
+     auto
+  have [refine0]: \<open>RETURN (b = RESTART) \<le> \<Down>bool_rel (restart_required_l a' c d)\<close>
+    if \<open>(b, b') \<in> ?GC a c'\<close> \<open>(a, a') \<in> ?R\<close> \<open>(c, c') \<in> nat_rel\<close>
+    for a a' b b' c c' d d' e e'
+    using that
+    unfolding restart_required_l_def
+    by refine_rcg auto
+  show ?thesis
+    unfolding uncurry_def restart_prog_wl_alt_def restart_prog_l_def rewatch_clauses_def
+    apply (intro frefI nres_relI)
+    apply (refine_rcg
+      cdcl_twl_restart_wl_prog_cdcl_twl_restart_l_prog[THEN fref_to_Down]
+      cdcl_twl_full_restart_wl_GC_prog[THEN fref_to_Down]
+      cdcl_twl_full_restart_wl_prog_cdcl_full_twl_restart_l_prog[THEN fref_to_Down])
+    subgoal unfolding restart_abs_wl_pre_def
+       by (fastforce simp: correct_watching_correct_watching)
+    subgoal by auto
+    subgoal by auto
+    subgoal by auto
+    apply assumption+
+    subgoal by auto
+    subgoal by auto
+    subgoal by auto
+    subgoal by (auto simp: correct_watching_correct_watching restart_abs_wl_pre_blits_in_\<L>\<^sub>i\<^sub>n)
+    subgoal by (auto simp: correct_watching_correct_watching restart_abs_wl_pre_blits_in_\<L>\<^sub>i\<^sub>n)
+    subgoal by auto
+    subgoal by (auto)
+    subgoal by auto
+    subgoal by (auto simp: correct_watching_correct_watching restart_abs_wl_pre_blits_in_\<L>\<^sub>i\<^sub>n)
+    subgoal by auto
+    subgoal by (auto simp: correct_watching_correct_watching restart_abs_wl_pre_blits_in_\<L>\<^sub>i\<^sub>n)
+    done
+qed
+
+
+definition (in twl_restart_ops) cdcl_twl_stgy_restart_prog_wl
+  :: \<open>'v twl_st_wl \<Rightarrow> 'v twl_st_wl nres\<close>
+where
+  \<open>cdcl_twl_stgy_restart_prog_wl (S\<^sub>0::'v twl_st_wl) =
+  do {
+    (brk, T, _, _, _) \<leftarrow> WHILE\<^sub>T\<^bsup>cdcl_twl_stgy_restart_abs_wl_inv S\<^sub>0\<^esup>
+      (\<lambda>(brk, _). \<not>brk)
+      (\<lambda>(brk, S, last_GC, last_Restart, n).
+      do {
+        T \<leftarrow> unit_propagation_outer_loop_wl S;
+        (brk, T) \<leftarrow> cdcl_twl_o_prog_wl T;
+        (T, last_GC, last_Restart, n) \<leftarrow> restart_prog_wl T last_GC last_Restart n brk;
+        RETURN (brk \<or> get_conflict_wl T \<noteq> None, T, last_GC, last_Restart, n)
+      })
+      (False, S\<^sub>0::'v twl_st_wl, size (get_all_learned_clss_wl S\<^sub>0), size (get_all_learned_clss_wl S\<^sub>0), 0);
+    RETURN T
+  }\<close>
+
+
+lemma cdcl_twl_stgy_restart_prog_wl_cdcl_twl_stgy_restart_prog_l:
+  \<open>(cdcl_twl_stgy_restart_prog_wl, cdcl_twl_stgy_restart_prog_l)
+    \<in> {(S, T).  (S, T) \<in> state_wl_l None \<and> correct_watching S \<and> blits_in_\<L>\<^sub>i\<^sub>n S} \<rightarrow>\<^sub>f
+      \<langle>{(S, T).  (S, T) \<in> state_wl_l None \<and> correct_watching S \<and> blits_in_\<L>\<^sub>i\<^sub>n S}\<rangle>nres_rel\<close>
+  (is \<open>_ \<in> ?R \<rightarrow>\<^sub>f \<langle>?S\<rangle>nres_rel\<close>)
+proof -
+  have [refine0]:
+    \<open>(x, y) \<in> ?R \<Longrightarrow> ((False, x, 0), False, y, 0) \<in> bool_rel \<times>\<^sub>r ?R \<times>\<^sub>r nat_rel\<close> for x y
+    by auto
+  show ?thesis
+    unfolding cdcl_twl_stgy_restart_prog_wl_def cdcl_twl_stgy_restart_prog_l_def
+    apply (intro frefI nres_relI)
+    apply (refine_rcg WHILEIT_refine[where
+      R=\<open>bool_rel \<times>\<^sub>r {(S, T).  (S, T) \<in> state_wl_l None \<and> correct_watching S \<and> blits_in_\<L>\<^sub>i\<^sub>n S} \<times>\<^sub>r nat_rel \<times>\<^sub>r nat_rel \<times>\<^sub>r nat_rel\<close>]
+      unit_propagation_outer_loop_wl_spec[THEN fref_to_Down]
+      cdcl_twl_full_restart_wl_prog_cdcl_twl_restart_l_prog[THEN fref_to_Down_curry4]
+      cdcl_twl_o_prog_wl_spec[THEN fref_to_Down])
+    subgoal by auto
+    subgoal for S T U V
+      unfolding cdcl_twl_stgy_restart_abs_wl_inv_def case_prod_beta
+      by (fastforce simp: prod_rel_fst_snd_iff)
+    subgoal by auto
+    subgoal by auto
+    subgoal by auto
+    subgoal by (auto simp: correct_watching_correct_watching)
+    subgoal by auto
+    done
+qed
+
+
+end
+
+end
